@prefix : <https://dmikhaylova.github.io/itdt_ontology/#> .
@prefix dc: <http://purl.org/dc/elements/1.1/> .
@prefix wd: <https://www.wikidata.org/wiki/> .
@prefix owl: <http://www.w3.org/2002/07/owl#> .
@prefix rdf: <http://www.w3.org/1999/02/22-rdf-syntax-ns#> .
@prefix xml: <http://www.w3.org/XML/1998/namespace/> .
@prefix xsd: <http://www.w3.org/2001/XMLSchema#> .
@prefix itdt: <http://www.semanticweb.org/daria/dt_archive#> .
@prefix rdfs: <http://www.w3.org/2000/01/rdf-schema#> .
@prefix rico: <https://www.ica.org/standards/RiC/ontology#> .
@prefix dcterms: <http://purl.org/dc/terms/> .
@base <https://dmikhaylova.github.io/itdt_ontology> .

<https://dmikhaylova.github.io/itdt_ontology> rdf:type owl:Ontology ;
                                               dc:creator "Daria Mikhaylova (University of Pisa)"@en ;
                                               dcterms:contributor "Daniele Metilli (University College London)"@en ;
                                               <http://purl.org/vocab/vann/preferredNamespacePrefix> "itdt"@en ;
                                               rdfs:comment """The ITDT ontology is an extension of RiC-O (https://www.ica.org/standards/RiC/ontology) created to describe the architectural records of the Italian architect and engineer Dino Tamburini. 
The ontology provides sub-classes of the class rico:Record for description of architectural graphical documents. 
The main concept of the ontology is the Architectural Project, which is seen from three different perspectives: that of file, that of knowledge process and that of potential built work."""@en ;
                                               rdfs:label "ITDT Ontology: Extension of RiC Ontology for architectural archives (version 0.1)"@en ;
                                               owl:versionInfo "version 0.1, 2022-07-17"@en .

#################################################################
#    Annotation properties
#################################################################

###  http://purl.org/dc/elements/1.1/creator
dc:creator rdf:type owl:AnnotationProperty .


###  http://purl.org/dc/elements/1.1/title
dc:title rdf:type owl:AnnotationProperty .


###  http://purl.org/dc/terms/contributor
dcterms:contributor rdf:type owl:AnnotationProperty .


###  http://purl.org/vocab/vann/preferredNamespacePrefix
<http://purl.org/vocab/vann/preferredNamespacePrefix> rdf:type owl:AnnotationProperty .


###  http://www.w3.org/2002/07/owl#sameAs
owl:sameAs rdf:type owl:AnnotationProperty .


###  http://www.w3.org/2004/02/skos/core#broader
<http://www.w3.org/2004/02/skos/core#broader> rdf:type owl:AnnotationProperty .


###  http://www.w3.org/2004/02/skos/core#changeNote
<http://www.w3.org/2004/02/skos/core#changeNote> rdf:type owl:AnnotationProperty .


###  http://www.w3.org/2004/02/skos/core#definition
<http://www.w3.org/2004/02/skos/core#definition> rdf:type owl:AnnotationProperty .


###  http://www.w3.org/2004/02/skos/core#example
<http://www.w3.org/2004/02/skos/core#example> rdf:type owl:AnnotationProperty .


###  http://www.w3.org/2004/02/skos/core#inScheme
<http://www.w3.org/2004/02/skos/core#inScheme> rdf:type owl:AnnotationProperty .


###  http://www.w3.org/2004/02/skos/core#narrower
<http://www.w3.org/2004/02/skos/core#narrower> rdf:type owl:AnnotationProperty .


###  http://www.w3.org/2004/02/skos/core#prefLabel
<http://www.w3.org/2004/02/skos/core#prefLabel> rdf:type owl:AnnotationProperty .


###  http://www.w3.org/2004/02/skos/core#scopeNote
<http://www.w3.org/2004/02/skos/core#scopeNote> rdf:type owl:AnnotationProperty .


###  https://www.ica.org/standards/RiC/ontology#RiCCMCorrespondingComponent
rico:RiCCMCorrespondingComponent rdf:type owl:AnnotationProperty .


###  https://www.ica.org/standards/RiC/ontology#closeTo
rico:closeTo rdf:type owl:AnnotationProperty .


#################################################################
#    Object Properties
#################################################################

###  https://dmikhaylova.github.io/itdt_ontology/#hasFormalBuildingType
:hasFormalBuildingType rdf:type owl:ObjectProperty ;
                       rdfs:subPropertyOf rico:hasOrHadCategory ;
                       owl:inverseOf :isFormalBuildingTypeOf ;
                       rdfs:domain :ArchitecturalProject ;
                       rdfs:range :FormalBuildingType ;
                       rdfs:comment "Connects an Architectural Project to its Formal Building Type."@en ;
                       rdfs:label "has formal building type"@en .


###  https://dmikhaylova.github.io/itdt_ontology/#hasFunctionalBuildingType
:hasFunctionalBuildingType rdf:type owl:ObjectProperty ;
                           rdfs:subPropertyOf rico:hasOrHadCategory ;
                           owl:inverseOf :isFunctionalBuildingTypeOf ;
                           rdfs:domain :ArchitecturalProject ;
                           rdfs:range :FunctionalBuildingType ;
                           rdfs:comment "Connects an Architectural Project to its Functional Building Type."@en ;
                           rdfs:label "has functional building type"@en .


###  https://dmikhaylova.github.io/itdt_ontology/#hasOrHadProjectPhase
:hasOrHadProjectPhase rdf:type owl:ObjectProperty ;
                      rdfs:subPropertyOf rico:hasOrHadPart ;
                      owl:inverseOf :isOrWasProjectPhaseOf ;
                      rdfs:domain :ArchitecturalProject ;
                      rdfs:range :ProjectPhase ;
                      rdfs:comment "Connects an Architectural Project to its Project Phase"@en ;
                      rdfs:label "has or had project phase"@en .


###  https://dmikhaylova.github.io/itdt_ontology/#hasOrHadProjectRole
:hasOrHadProjectRole rdf:type owl:ObjectProperty ;
                     rdfs:subPropertyOf rico:isRelatedTo ;
                     owl:inverseOf :isOrWasProjectRoleOf ;
                     rdfs:domain :ProjectParticipation ;
                     rdfs:range :ProjectRole ;
                     rdfs:comment "Connects Project Participation with the Project Role the Agent had in the Architectural Project."@en ;
                     rdfs:label "has or had project role"@en .


###  https://dmikhaylova.github.io/itdt_ontology/#hasOrHasProjectParticipation
:hasOrHasProjectParticipation rdf:type owl:ObjectProperty ;
                              rdfs:subPropertyOf rico:isEventAssociatedWith ;
                              owl:inverseOf :isOrWasProjectParticipationOf ;
                              rdfs:domain rico:Activity ;
                              rdfs:range :ProjectParticipation ;
                              rdfs:comment "Connects an Architectural Project o Project Phase to a Project Participation."@en ;
                              rdfs:label "has or had project participation"@en .


###  https://dmikhaylova.github.io/itdt_ontology/#hasProjectScale
:hasProjectScale rdf:type owl:ObjectProperty ;
                 rdfs:subPropertyOf rico:hasOrHadCategory ;
                 owl:inverseOf :isProjectScaleOf ;
                 rdfs:domain :ArchitecturalProject ;
                 rdfs:range :ProjectScale ;
                 rdfs:comment "Connects an Architectural Project to its Project Scale"@en ;
                 rdfs:label "has project scale"@en .


###  https://dmikhaylova.github.io/itdt_ontology/#isCommissionedBy
:isCommissionedBy rdf:type owl:ObjectProperty ;
                  rdfs:subPropertyOf rico:hasProvenance ;
                  owl:inverseOf :isCommissionerOf ;
                  rdfs:domain :ArchitecturalProject ;
                  rdfs:range rico:Agent ;
                  rdfs:comment "Connects an Architectural Project to an Agent that commissioned its realisation."@en ;
                  rdfs:label "is commissioned by"@en .


###  https://dmikhaylova.github.io/itdt_ontology/#isCommissionerOf
:isCommissionerOf rdf:type owl:ObjectProperty ;
                  rdfs:subPropertyOf rico:isProvenanceOf ;
                  rdfs:domain rico:Agent ;
                  rdfs:range :ArchitecturalProject ;
                  rdfs:comment "Connects an Agent to an Architectural project that they commissioned."@en ;
                  rdfs:label "is commissioner of"@en .


###  https://dmikhaylova.github.io/itdt_ontology/#isFormalBuildingTypeOf
:isFormalBuildingTypeOf rdf:type owl:ObjectProperty ;
                        rdfs:subPropertyOf rico:isOrWasCategoryOf ;
                        rdfs:domain :FormalBuildingType ;
                        rdfs:range :ArchitecturalProject ;
                        rdfs:comment "Connects a Formal Building Type to an Architectural Project that it categorises."@en ;
                        rdfs:label "is formal building type of"@en .


###  https://dmikhaylova.github.io/itdt_ontology/#isFunctionalBuildingTypeOf
:isFunctionalBuildingTypeOf rdf:type owl:ObjectProperty ;
                            rdfs:subPropertyOf rico:isOrWasCategoryOf ;
                            rdfs:domain :FunctionalBuildingType ;
                            rdfs:range :ArchitecturalProject ;
                            rdfs:comment "Connects a Functional Building Type to an Architectural Project that it categorises."@en ;
                            rdfs:label "is functional building type of"@en .


###  https://dmikhaylova.github.io/itdt_ontology/#isOrWasDescribedBy
:isOrWasDescribedBy rdf:type owl:ObjectProperty ;
                    rdfs:subPropertyOf rico:isOrWasSubjectOf ;
                    owl:inverseOf rico:describesOrDescribed ;
                    rdfs:range rico:RecordResource ;
                    rdfs:comment "inverse of describes or described"@en ;
                    rdfs:label "is or was described by"@en .


###  https://dmikhaylova.github.io/itdt_ontology/#isOrWasProjectParticipationOf
:isOrWasProjectParticipationOf rdf:type owl:ObjectProperty ;
                               rdfs:subPropertyOf rico:isAssociatedWithEvent ;
                               rdfs:domain :ProjectParticipation ;
                               rdfs:range rico:Activity ;
                               rdfs:comment "Connects Project Participation to an Architectural Project or to a Project Phase in which an Agent participated with a specific Project Role"@en ;
                               rdfs:label "is or was project participation of"@en .


###  https://dmikhaylova.github.io/itdt_ontology/#isOrWasProjectPhaseOf
:isOrWasProjectPhaseOf rdf:type owl:ObjectProperty ;
                       rdfs:subPropertyOf rico:isOrWasPartOf ;
                       rdfs:domain :ProjectPhase ;
                       rdfs:range :ArchitecturalProject ;
                       rdfs:comment "Connects a Project Phase to an Architectural Project of which it was part."@en ;
                       rdfs:label "is or was project phase of"@en .


###  https://dmikhaylova.github.io/itdt_ontology/#isOrWasProjectRoleOf
:isOrWasProjectRoleOf rdf:type owl:ObjectProperty ;
                      rdfs:subPropertyOf rico:isRelatedTo ;
                      rdfs:domain :ProjectRole ;
                      rdfs:range :ProjectParticipation ;
                      rdfs:comment "Connects a Project Participation to a Project Role with which an Agent participated in a Architectural project connected by the same Project Participation."@en ;
                      rdfs:label "is or was project role of"@en .


###  https://dmikhaylova.github.io/itdt_ontology/#isProjectScaleOf
:isProjectScaleOf rdf:type owl:ObjectProperty ;
                  rdfs:subPropertyOf rico:isOrWasCategoryOf ;
                  rdfs:domain :ProjectScale ;
                  rdfs:range :ArchitecturalProject ;
                  rdfs:comment "Connects a Project Scale to an Architectural Project that it categorises."@en ;
                  rdfs:label "is project scale of"@en .


###  https://www.ica.org/standards/RiC/ontology#containsOrContained
rico:containsOrContained rdf:type owl:ObjectProperty ;
                         rdfs:subPropertyOf rico:hasOrHadPart ,
                                            rico:isAssociatedWithPlace ;
                         owl:inverseOf rico:isOrWasContainedBy ;
                         rdfs:domain rico:Place ;
                         rdfs:range rico:Place ;
                         rdfs:comment """Connects a Place to a region that is or was within
            it."""@en ;
                         rdfs:isDefinedBy <https://www.ica.org/standards/RiC/ontology> ;
                         rdfs:label "contains or contained"@en ;
                         <http://www.w3.org/2004/02/skos/core#changeNote> [ ] ;
<http://www.w3.org/2004/02/skos/core#scopeNote> """Use for connecting two geographical or administrative
            regions."""@en ;
rico:RiCCMCorrespondingComponent """RiC-R007 ('contains or contained'
            relation)"""@en .


###  https://www.ica.org/standards/RiC/ontology#describesOrDescribed
rico:describesOrDescribed rdf:type owl:ObjectProperty ;
                          rdfs:subPropertyOf rico:hasOrHadSubject ;
                          rdfs:domain rico:RecordResource ;
                          rdfs:comment """Connects a Record Resource to a Thing that it
            describes."""@en ;
                          rdfs:isDefinedBy <https://www.ica.org/standards/RiC/ontology> ;
                          rdfs:label "describes or described"@en ;
                          <http://www.w3.org/2004/02/skos/core#changeNote> [ ] ;
<http://www.w3.org/2004/02/skos/core#scopeNote> """Can be used, among other situations, for specifying that some
            finding aid (a Record that has Documentary Form Type Finding Aid) describes some Record
            Set."""@en ;
rico:RiCCMCorrespondingComponent """RiC-R021 (describes or
            described)"""@en .


###  https://www.ica.org/standards/RiC/ontology#documentedBy
rico:documentedBy rdf:type owl:ObjectProperty ;
                  rdfs:subPropertyOf rico:resultsOrResultedIn ;
                  owl:inverseOf rico:documents ;
                  rdfs:domain rico:Activity ;
                  rdfs:range [ rdf:type owl:Class ;
                               owl:unionOf ( rico:Instantiation
                                             rico:RecordResource
                                           )
                             ] ;
                  rdfs:comment "Inverse of 'documents' object property."@en ;
                  rdfs:isDefinedBy <https://www.ica.org/standards/RiC/ontology> ;
                  rdfs:label "documented by"@en ;
                  <http://www.w3.org/2004/02/skos/core#changeNote> [ ] ;
rico:RiCCMCorrespondingComponent """RiC-R033i ('documented by'
            relation)"""@en .


###  https://www.ica.org/standards/RiC/ontology#documents
rico:documents rdf:type owl:ObjectProperty ;
               rdfs:subPropertyOf rico:resultsOrResultedFrom ;
               rdfs:domain [ rdf:type owl:Class ;
                             owl:unionOf ( rico:Instantiation
                                           rico:RecordResource
                                         )
                           ] ;
               rdfs:range rico:Activity ;
               owl:propertyChainAxiom ( rico:documents
                                        :isOrWasProjectPhaseOf
                                      ) ;
               rdfs:comment """Connects a Record Resource or an Instantiation to the Activity
            that generates the Record Resource or Instantiation."""@en ;
               rdfs:isDefinedBy <https://www.ica.org/standards/RiC/ontology> ;
               rdfs:label "documents"@en ;
               <http://www.w3.org/2004/02/skos/core#changeNote> [ ] ;
rico:RiCCMCorrespondingComponent """RiC-R033 ('documents'
            relation)"""@en .


###  https://www.ica.org/standards/RiC/ontology#followsInTime
rico:followsInTime rdf:type owl:ObjectProperty ;
                   rdfs:subPropertyOf rico:followsOrFollowed ;
                   owl:inverseOf rico:precedesInTime ;
                   rdfs:label "follows in time"@en .


###  https://www.ica.org/standards/RiC/ontology#followsOrFollowed
rico:followsOrFollowed rdf:type owl:ObjectProperty ;
                       rdfs:subPropertyOf rico:isRelatedTo ;
                       owl:inverseOf rico:precedesOrPreceded ;
                       rdfs:comment "Inverse of 'precedesOrPreceded' object property."@en ;
                       rdfs:isDefinedBy <https://www.ica.org/standards/RiC/ontology> ;
                       rdfs:label "follows or followed"@en ;
                       <http://www.w3.org/2004/02/skos/core#changeNote> [ ] ;
rico:RiCCMCorrespondingComponent """RiC-R008i ('follows or followed'
            relation)"""@en .


###  https://www.ica.org/standards/RiC/ontology#hasAuthor
rico:hasAuthor rdf:type owl:ObjectProperty ;
               rdfs:subPropertyOf rico:hasCreator ;
               owl:inverseOf rico:isAuthorOf ;
               rdfs:domain rico:Record ;
               rdfs:comment """Connects a Record to the Group, Person or Position that is
            responsible for conceiving and formulating the information contained in the
            Record."""@en ;
               rdfs:isDefinedBy <https://www.ica.org/standards/RiC/ontology> ;
               rdfs:label "has author"@en ;
               <http://www.w3.org/2004/02/skos/core#changeNote> [ ] ;
<http://www.w3.org/2004/02/skos/core#scopeNote> """To be used for any contribution to the content of a Record.
            Includes (of course) the Person, Group or Position in whose name or by whose command the
            content may have been formulated and first instantiated (e.g. the person who signed
            it)."""@en ;
rico:RiCCMCorrespondingComponent """RiC-R079 ('has author'
            relation)"""@en .


###  https://www.ica.org/standards/RiC/ontology#hasBeginningDate
rico:hasBeginningDate rdf:type owl:ObjectProperty ;
                      rdfs:subPropertyOf rico:isAssociatedWithDate ;
                      owl:inverseOf rico:isBeginningDateOf ;
                      rdfs:range rico:Date ;
                      rdfs:comment "Inverse of 'is beginning date of' object property"@en ;
                      rdfs:isDefinedBy <https://www.ica.org/standards/RiC/ontology> ;
                      rdfs:label "has beginning date "@en ;
                      rico:RiCCMCorrespondingComponent """RiC-R069i ('has beginning date'
            relation)"""@en .


###  https://www.ica.org/standards/RiC/ontology#hasBirthDate
rico:hasBirthDate rdf:type owl:ObjectProperty ;
                  rdfs:subPropertyOf rico:hasBeginningDate ;
                  owl:inverseOf rico:isBirthDateOf ;
                  rdfs:domain rico:Person ;
                  rdfs:range rico:Date ;
                  rdfs:comment "Inverse of 'is birth date of' object property"@en ;
                  rdfs:isDefinedBy <https://www.ica.org/standards/RiC/ontology> ;
                  rdfs:label "has birth date "@en ;
                  rico:RiCCMCorrespondingComponent """RiC-R070i ('has birth date'
            relation)"""@en .


###  https://www.ica.org/standards/RiC/ontology#hasCreator
rico:hasCreator rdf:type owl:ObjectProperty ;
                rdfs:subPropertyOf rico:hasProvenance ;
                owl:inverseOf rico:isCreatorOf ;
                rdfs:domain [ rdf:type owl:Class ;
                              owl:unionOf ( rico:Instantiation
                                            rico:RecordResource
                                          )
                            ] ;
                rdfs:range rico:Agent ;
                rdfs:comment """Connects a Record Resource or an Instantiation to an Agent that
            is either responsible for all or some of the content of the Record Resource or is a
            contributor to the genesis or production of an Instantiation."""@en ;
                rdfs:isDefinedBy <https://www.ica.org/standards/RiC/ontology> ;
                rdfs:label "has creator"@en ;
                <http://www.w3.org/2004/02/skos/core#changeNote> [ ] ;
<http://www.w3.org/2004/02/skos/core#scopeNote> """Covers the definition of author in diplomatics, and any
            contribution to the intellectual content of a Record Resource."""@en ;
rico:RiCCMCorrespondingComponent """RiC-R027 ('has creator'
            relation)"""@en .


###  https://www.ica.org/standards/RiC/ontology#hasDeathDate
rico:hasDeathDate rdf:type owl:ObjectProperty ;
                  rdfs:subPropertyOf rico:hasEndDate ;
                  owl:inverseOf rico:isDeathDateOf ;
                  rdfs:domain rico:Person ;
                  rdfs:range rico:Date ;
                  rdfs:comment "Inverse of 'is death date of' object property"@en ;
                  rdfs:isDefinedBy <https://www.ica.org/standards/RiC/ontology> ;
                  rdfs:label "has death date "@en ;
                  rico:RiCCMCorrespondingComponent """RiC-R072i ('has death date'
            relation)"""@en .


###  https://www.ica.org/standards/RiC/ontology#hasDerivedInstantiation
rico:hasDerivedInstantiation rdf:type owl:ObjectProperty ;
                             rdfs:subPropertyOf rico:precedesInTime ;
                             owl:inverseOf rico:isDerivedFromInstantiation ;
                             rdfs:domain rico:Instantiation ;
                             rdfs:range rico:Instantiation ;
                             rdfs:comment """Connects an Instantiation to an Instantiation that is derived
            from it."""@en ;
                             rdfs:isDefinedBy <https://www.ica.org/standards/RiC/ontology> ;
                             rdfs:label "has derived instantiation "@en ;
                             rico:RiCCMCorrespondingComponent """RiC-R014 ('has derived instantiation'
            relation)"""@en .


###  https://www.ica.org/standards/RiC/ontology#hasDocumentaryFormType
rico:hasDocumentaryFormType rdf:type owl:ObjectProperty ;
                            rdfs:subPropertyOf rico:hasOrHadCategory ;
                            owl:inverseOf rico:isDocumentaryFormTypeOf ;
                            rdfs:domain [ rdf:type owl:Class ;
                                          owl:unionOf ( rico:Record
                                                        rico:RecordPart
                                                      )
                                        ] ;
                            rdfs:range rico:DocumentaryFormType ;
                            rdfs:comment """Connects a Record or Record Part to its Documentary Form
            Type."""@en ;
                            rdfs:isDefinedBy <https://www.ica.org/standards/RiC/ontology> ;
                            rdfs:label "has documentary form type"@en ;
                            <http://www.w3.org/2004/02/skos/core#changeNote> [ ] .


###  https://www.ica.org/standards/RiC/ontology#hasEndDate
rico:hasEndDate rdf:type owl:ObjectProperty ;
                rdfs:subPropertyOf rico:isAssociatedWithDate ;
                owl:inverseOf rico:isEndDateOf ;
                rdfs:range rico:Date ;
                rdfs:comment "Inverse of 'is end date of' object property."@en ;
                rdfs:isDefinedBy <https://www.ica.org/standards/RiC/ontology> ;
                rdfs:label "has end date "@en ;
                rico:RiCCMCorrespondingComponent """RiC-R071i ('has end date'
            relation)"""@en .


###  https://www.ica.org/standards/RiC/ontology#hasInstantiation
rico:hasInstantiation rdf:type owl:ObjectProperty ;
                      rdfs:subPropertyOf rico:isRelatedTo ;
                      owl:inverseOf rico:isInstantiationOf ;
                      rdfs:domain rico:RecordResource ;
                      rdfs:range rico:Instantiation ;
                      rdfs:comment """Connects a Record Resource to one of its
            Instantiations."""@en ;
                      rdfs:isDefinedBy <https://www.ica.org/standards/RiC/ontology> ;
                      rdfs:label "has instantiation"@en ;
                      <http://www.w3.org/2004/02/skos/core#changeNote> [ ] ,
[ ] ;
rico:RiCCMCorrespondingComponent """RiC-R025 ('has instantiation'
            relation)"""@en .


###  https://www.ica.org/standards/RiC/ontology#hasOrHadAuthorityOver
rico:hasOrHadAuthorityOver rdf:type owl:ObjectProperty ;
                           rdfs:subPropertyOf rico:isRelatedTo ;
                           owl:inverseOf rico:isOrWasUnderAuthorityOf ;
                           rdfs:domain rico:Agent ;
                           rdfs:comment """Connects an Agent to a Thing the Agent has or had authority
            over."""@en ;
                           rdfs:isDefinedBy <https://www.ica.org/standards/RiC/ontology> ;
                           rdfs:label "has or had authority over"@en ;
                           <http://www.w3.org/2004/02/skos/core#changeNote> [ ] ;
rico:RiCCMCorrespondingComponent """RiC-R036 ('has or had authority over'
            relation)"""@en .


###  https://www.ica.org/standards/RiC/ontology#hasOrHadCategory
rico:hasOrHadCategory rdf:type owl:ObjectProperty ;
                      rdfs:subPropertyOf rico:isRelatedTo ;
                      owl:inverseOf rico:isOrWasCategoryOf ;
                      rdfs:domain rico:Thing ;
                      rdfs:range rico:Type ;
                      rdfs:comment """Connects a Thing to a Type that categorizes or categorized
            it."""@en ;
                      rdfs:isDefinedBy <https://www.ica.org/standards/RiC/ontology> ;
                      rdfs:label "has or had category"@en ;
                      <http://www.w3.org/2004/02/skos/core#changeNote> [ ] .


###  https://www.ica.org/standards/RiC/ontology#hasOrHadController
rico:hasOrHadController rdf:type owl:ObjectProperty ;
                        rdfs:subPropertyOf rico:isOrWasUnderAuthorityOf ;
                        owl:inverseOf rico:isOrWasControllerOf ;
                        rdfs:domain rico:Agent ;
                        rdfs:range rico:Agent ;
                        rdfs:comment """Inverse of 'is or was controller of' object
            property."""@en ;
                        rdfs:isDefinedBy <https://www.ica.org/standards/RiC/ontology> ;
                        rdfs:label "has or had controller"@en ;
                        <http://www.w3.org/2004/02/skos/core#changeNote> [ ] ;
rico:RiCCMCorrespondingComponent """RiC-R041i ('has or had controller'
            relation)"""@en .


###  https://www.ica.org/standards/RiC/ontology#hasOrHadLeader
rico:hasOrHadLeader rdf:type owl:ObjectProperty ;
                    rdfs:subPropertyOf rico:hasOrHadController ;
                    owl:inverseOf rico:isOrWasLeaderOf ;
                    rdfs:domain rico:Group ;
                    rdfs:range rico:Person ;
                    rdfs:comment "Inverse of 'is or was leader of' object property."@en ;
                    rdfs:isDefinedBy <https://www.ica.org/standards/RiC/ontology> ;
                    rdfs:label "has or had leader"@en ;
                    <http://www.w3.org/2004/02/skos/core#changeNote> [ ] ;
rico:RiCCMCorrespondingComponent """RiC-R042i ('has or had leader'
            relation)"""@en .


###  https://www.ica.org/standards/RiC/ontology#hasOrHadMainSubject
rico:hasOrHadMainSubject rdf:type owl:ObjectProperty ;
                         rdfs:subPropertyOf rico:hasOrHadSubject ;
                         owl:inverseOf rico:isOrWasMainSubjectOf ;
                         rdfs:domain rico:RecordResource ;
                         rdfs:comment """Connects a Record Resource to a Thing that is or was its main
            subject."""@en ;
                         rdfs:isDefinedBy <https://www.ica.org/standards/RiC/ontology> ;
                         rdfs:label "has or had main subject"@en ;
                         <http://www.w3.org/2004/02/skos/core#changeNote> [ ] ;
<http://www.w3.org/2004/02/skos/core#scopeNote> """Use for specifying, for example, that a Record Set of type
            personal file has main subject some person, which would help end users to retrieve the
            main archival resources about this person."""@en ;
rico:RiCCMCorrespondingComponent """RiC-R020 ('has or had main subject'
            relation)"""@en .


###  https://www.ica.org/standards/RiC/ontology#hasOrHadOwner
rico:hasOrHadOwner rdf:type owl:ObjectProperty ;
                   rdfs:subPropertyOf rico:isOrWasUnderAuthorityOf ;
                   owl:inverseOf rico:isOrWasOwnerOf ;
                   rdfs:comment "Inverse of 'is or was owner of' object property."@en ;
                   rdfs:isDefinedBy <https://www.ica.org/standards/RiC/ontology> ;
                   rdfs:label "has or had owner"@en ;
                   <http://www.w3.org/2004/02/skos/core#changeNote> [ ] ;
rico:RiCCMCorrespondingComponent """RiC-R037i ('has or had owner'
            relation)"""@en .


###  https://www.ica.org/standards/RiC/ontology#hasOrHadPart
rico:hasOrHadPart rdf:type owl:ObjectProperty ;
                  rdfs:subPropertyOf rico:isRelatedTo ;
                  owl:inverseOf rico:isOrWasPartOf ;
                  rdfs:comment "Connects a Thing to a constitutive or component part of that Thing."@en ;
                  rdfs:label "has or had part"@en .


###  https://www.ica.org/standards/RiC/ontology#hasOrHadParticipant
rico:hasOrHadParticipant rdf:type owl:ObjectProperty ;
                         rdfs:subPropertyOf rico:isEventAssociatedWith ;
                         owl:inverseOf rico:isOrWasParticipantIn ;
                         rdfs:domain rico:Event ;
                         rdfs:comment """Connects an Event to a Thing that is or was actively or
            passively involved in it."""@en ;
                         rdfs:isDefinedBy <https://www.ica.org/standards/RiC/ontology> ;
                         rdfs:label "has or had participant"@en ;
                         <http://www.w3.org/2004/02/skos/core#changeNote> [ ] ;
rico:RiCCMCorrespondingComponent """RiC-R058 ('has or had participant'
            relation)"""@en .


###  https://www.ica.org/standards/RiC/ontology#hasOrHadSubject
rico:hasOrHadSubject rdf:type owl:ObjectProperty ;
                     rdfs:subPropertyOf rico:isRelatedTo ;
                     owl:inverseOf rico:isOrWasSubjectOf ;
                     rdfs:domain rico:RecordResource ;
                     rdfs:comment """Connects a Record Resource to a Thing that is or was its
            subject."""@en ;
                     rdfs:isDefinedBy <https://www.ica.org/standards/RiC/ontology> ;
                     rdfs:label "has or had subject"@en ;
                     <http://www.w3.org/2004/02/skos/core#changeNote> [ ] ;
rico:RiCCMCorrespondingComponent """RiC-R019 ('has or had subject'
            relation)"""@en .


###  https://www.ica.org/standards/RiC/ontology#hasOrHadSubordinate
rico:hasOrHadSubordinate rdf:type owl:ObjectProperty ;
                         rdfs:subPropertyOf rico:isAgentAssociatedWithAgent ;
                         rdfs:label "has or had subordinate"@en .


###  https://www.ica.org/standards/RiC/ontology#hasProvenance
rico:hasProvenance rdf:type owl:ObjectProperty ;
                   rdfs:subPropertyOf rico:isRelatedTo ;
                   owl:inverseOf rico:isProvenanceOf ;
                   rdfs:domain [ rdf:type owl:Class ;
                                 owl:unionOf ( rico:Instantiation
                                               rico:RecordResource
                                             )
                               ] ;
                   rdfs:range rico:Agent ;
                   rdfs:comment "Connects a Record Resource or an Instantiation to an Agent that creates or accumulates the Record Resource, receives it, or sends it." ;
                   rdfs:label "has provenance" .


###  https://www.ica.org/standards/RiC/ontology#hasRecordSetType
rico:hasRecordSetType rdf:type owl:ObjectProperty ;
                      rdfs:subPropertyOf rico:hasOrHadCategory ;
                      owl:inverseOf rico:isRecordSetTypeOf ;
                      rdfs:domain rico:RecordSet ;
                      rdfs:range rico:RecordSetType ;
                      rdfs:comment """Connects a Record Set to a Record Set Type that categorizes
            it."""@en ;
                      rdfs:isDefinedBy <https://www.ica.org/standards/RiC/ontology> ;
                      rdfs:label "has record set type"@en ;
                      <http://www.w3.org/2004/02/skos/core#changeNote> [ ] .


###  https://www.ica.org/standards/RiC/ontology#hasRepresentationType
rico:hasRepresentationType rdf:type owl:ObjectProperty ;
                           rdfs:subPropertyOf rico:hasOrHadCategory ;
                           owl:inverseOf rico:isRepresentationTypeOf ;
                           rdfs:domain rico:Instantiation ;
                           rdfs:range rico:RepresentationType ;
                           rdfs:comment """Connects an Instantiation to a Representation Type that
            categorizes its representation type."""@en ;
                           rdfs:isDefinedBy <https://www.ica.org/standards/RiC/ontology> ;
                           rdfs:label "has representation type"@en ;
                           <http://www.w3.org/2004/02/skos/core#changeNote> [ ] .


###  https://www.ica.org/standards/RiC/ontology#includesOrIncluded
rico:includesOrIncluded rdf:type owl:ObjectProperty ;
                        rdfs:subPropertyOf rico:isRecordResourceAssociatedWithRecordResource ;
                        owl:inverseOf rico:isOrWasIncludedIn ;
                        rdfs:domain rico:RecordSet ;
                        rdfs:range [ rdf:type owl:Class ;
                                     owl:unionOf ( rico:Record
                                                   rico:RecordSet
                                                 )
                                   ] ;
                        rdfs:comment """Connects a Record Set to a Record or Record Set it aggregates,
            or aggregated in the past."""@en ;
                        rdfs:isDefinedBy <https://www.ica.org/standards/RiC/ontology> ;
                        rdfs:label "includes or included"@en ;
                        <http://www.w3.org/2004/02/skos/core#changeNote> [ ] ;
<http://www.w3.org/2004/02/skos/core#scopeNote> """A Record or Record Set can be aggregated in one or many Record
            Sets simultaneously or through time"""@en ;
rico:RiCCMCorrespondingComponent """RiC-R024 ('includes or included'
            relation)"""@en .


###  https://www.ica.org/standards/RiC/ontology#isAgentAssociatedWithAgent
rico:isAgentAssociatedWithAgent rdf:type owl:ObjectProperty ;
                                rdfs:subPropertyOf rico:isRelatedTo ;
                                rdf:type owl:SymmetricProperty ;
                                rdfs:domain rico:Agent ;
                                rdfs:range rico:Agent ;
                                rdfs:comment """Connects two Agents. This object property is
            symmetric."""@en ;
                                rdfs:isDefinedBy <https://www.ica.org/standards/RiC/ontology> ;
                                rdfs:label "is agent associated with agent "@en ;
                                <http://www.w3.org/2004/02/skos/core#scopeNote> """Use to connect two Agents only if it is not possible to be
            more accurate and use a narrower Agent to Agent relation, e.g. ‘has work relation
            with’."""@en ;
                                rico:RiCCMCorrespondingComponent """RiC-R044 ('is agent associated with agent'
            relation)"""@en .


###  https://www.ica.org/standards/RiC/ontology#isAssociatedWithDate
rico:isAssociatedWithDate rdf:type owl:ObjectProperty ;
                          rdfs:subPropertyOf rico:isRelatedTo ;
                          owl:inverseOf rico:isDateAssociatedWith ;
                          rdfs:range rico:Date ;
                          rdfs:comment """Inverse of 'is date associated with' object
            property."""@en ;
                          rdfs:isDefinedBy <https://www.ica.org/standards/RiC/ontology> ;
                          rdfs:label "is associated with date "@en ;
                          rico:RiCCMCorrespondingComponent """RiC-R068i ('is associated with date'
            relation)"""@en .


###  https://www.ica.org/standards/RiC/ontology#isAssociatedWithEvent
rico:isAssociatedWithEvent rdf:type owl:ObjectProperty ;
                           rdfs:subPropertyOf rico:isRelatedTo ;
                           owl:inverseOf rico:isEventAssociatedWith ;
                           rdfs:range rico:Event ;
                           rdfs:comment """Inverse of 'is event associated with' object
            property."""@en ;
                           rdfs:isDefinedBy <https://www.ica.org/standards/RiC/ontology> ;
                           rdfs:label "is associated with event "@en ;
                           rico:RiCCMCorrespondingComponent """RiC-R057i ('is associated with event'
            relation)"""@en .


###  https://www.ica.org/standards/RiC/ontology#isAssociatedWithPlace
rico:isAssociatedWithPlace rdf:type owl:ObjectProperty ;
                           rdfs:subPropertyOf rico:isRelatedTo ;
                           owl:inverseOf rico:isPlaceAssociatedWith ;
                           rdfs:domain rico:Thing ;
                           rdfs:range rico:Place ;
                           rdfs:comment """Inverse of 'is place associated with' object
            property."""@en ;
                           rdfs:isDefinedBy <https://www.ica.org/standards/RiC/ontology> ;
                           rdfs:label "is associated with place "@en ;
                           rico:RiCCMCorrespondingComponent """RiC-R074i ('is associated with place'
            relation)"""@en .


###  https://www.ica.org/standards/RiC/ontology#isAuthorOf
rico:isAuthorOf rdf:type owl:ObjectProperty ;
                rdfs:subPropertyOf rico:isCreatorOf ;
                rdfs:range rico:Record ;
                rdfs:comment "Inverse of 'has author' object property."@en ;
                rdfs:isDefinedBy <https://www.ica.org/standards/RiC/ontology> ;
                rdfs:label "is author of"@en ;
                <http://www.w3.org/2004/02/skos/core#changeNote> [ ] ;
rico:RiCCMCorrespondingComponent """RiC-R079i ('is author of'
            relation)"""@en .


###  https://www.ica.org/standards/RiC/ontology#isBeginningDateOf
rico:isBeginningDateOf rdf:type owl:ObjectProperty ;
                       rdfs:subPropertyOf rico:isDateAssociatedWith ;
                       rdfs:domain rico:Date ;
                       rdfs:comment """Connects a Date to a Thing that came into existence on that
            Date."""@en ;
                       rdfs:isDefinedBy <https://www.ica.org/standards/RiC/ontology> ;
                       rdfs:label "is beginning date of "@en ;
                       rico:RiCCMCorrespondingComponent """RiC-R069 ('is beginning date of'
            relation)"""@en .


###  https://www.ica.org/standards/RiC/ontology#isBirthDateOf
rico:isBirthDateOf rdf:type owl:ObjectProperty ;
                   rdfs:subPropertyOf rico:isBeginningDateOf ;
                   rdfs:domain rico:Date ;
                   rdfs:range rico:Person ;
                   rdfs:comment """Connects a Date to a Person that was born on that
            Date."""@en ;
                   rdfs:isDefinedBy <https://www.ica.org/standards/RiC/ontology> ;
                   rdfs:label "is birth date of "@en ;
                   rico:RiCCMCorrespondingComponent """RiC-R070 ('is birth date of'
            relation)"""@en .


###  https://www.ica.org/standards/RiC/ontology#isCreatorOf
rico:isCreatorOf rdf:type owl:ObjectProperty ;
                 rdfs:subPropertyOf rico:isProvenanceOf ;
                 rdfs:domain rico:Agent ;
                 rdfs:range [ rdf:type owl:Class ;
                              owl:unionOf ( rico:Instantiation
                                            rico:RecordResource
                                          )
                            ] ;
                 rdfs:comment "Inverse of 'has creator' object property."@en ;
                 rdfs:isDefinedBy <https://www.ica.org/standards/RiC/ontology> ;
                 rdfs:label "is creator of"@en ;
                 <http://www.w3.org/2004/02/skos/core#changeNote> [ ] ;
rico:RiCCMCorrespondingComponent """RiC-R027i ('is creator of
            'relation')"""@en .


###  https://www.ica.org/standards/RiC/ontology#isDateAssociatedWith
rico:isDateAssociatedWith rdf:type owl:ObjectProperty ;
                          rdfs:subPropertyOf rico:isRelatedTo ;
                          rdfs:domain rico:Date ;
                          rdfs:comment """Connects a Date to a Thing that the Date is associated with the
            existence and lifecycle of."""@en ;
                          rdfs:isDefinedBy <https://www.ica.org/standards/RiC/ontology> ;
                          rdfs:label "is date associated with "@en ;
                          rico:RiCCMCorrespondingComponent """RiC-R068 ('is date associated with'
            relation)"""@en .


###  https://www.ica.org/standards/RiC/ontology#isDeathDateOf
rico:isDeathDateOf rdf:type owl:ObjectProperty ;
                   rdfs:subPropertyOf rico:isEndDateOf ;
                   rdfs:domain rico:Date ;
                   rdfs:range rico:Person ;
                   rdfs:comment """Connects a Date to a Person who died on that
            Date."""@en ;
                   rdfs:isDefinedBy <https://www.ica.org/standards/RiC/ontology> ;
                   rdfs:label "is death date of "@en ;
                   rico:RiCCMCorrespondingComponent """RiC-R072 ('is death date of'
            relation)"""@en .


###  https://www.ica.org/standards/RiC/ontology#isDerivedFromInstantiation
rico:isDerivedFromInstantiation rdf:type owl:ObjectProperty ;
                                rdfs:subPropertyOf rico:followsInTime ,
                                                   rico:isInstantiationAssociatedWithInstantiation ;
                                rdfs:domain rico:Instantiation ;
                                rdfs:range rico:Instantiation ;
                                rdfs:comment """Inverse of 'has derived instantiation' object
            property."""@en ;
                                rdfs:isDefinedBy <https://www.ica.org/standards/RiC/ontology> ;
                                rdfs:label "is derived from instantiation "@en ;
                                rico:RiCCMCorrespondingComponent """RiC-R014i ('is derived from instantiation'
            relation)"""@en .


###  https://www.ica.org/standards/RiC/ontology#isDocumentaryFormTypeOf
rico:isDocumentaryFormTypeOf rdf:type owl:ObjectProperty ;
                             rdfs:subPropertyOf rico:isOrWasCategoryOf ;
                             rdfs:domain rico:DocumentaryFormType ;
                             rdfs:range [ rdf:type owl:Class ;
                                          owl:unionOf ( rico:Record
                                                        rico:RecordPart
                                                      )
                                        ] ;
                             rdfs:comment """Connects a Documentary Form Type to a Record or Record Part that
            it categorizes."""@en ;
                             rdfs:isDefinedBy <https://www.ica.org/standards/RiC/ontology> ;
                             rdfs:label "is documentary form type of"@en ;
                             <http://www.w3.org/2004/02/skos/core#changeNote> [ ] .


###  https://www.ica.org/standards/RiC/ontology#isEndDateOf
rico:isEndDateOf rdf:type owl:ObjectProperty ;
                 rdfs:subPropertyOf rico:isDateAssociatedWith ;
                 rdfs:domain rico:Date ;
                 rdfs:comment """Connects a Date to a Thing whose existence ended on that
            Date."""@en ;
                 rdfs:isDefinedBy <https://www.ica.org/standards/RiC/ontology> ;
                 rdfs:label "is end date of "@en ;
                 rico:RiCCMCorrespondingComponent """RiC-R071 ('is end date
            of')"""@en .


###  https://www.ica.org/standards/RiC/ontology#isEventAssociatedWith
rico:isEventAssociatedWith rdf:type owl:ObjectProperty ;
                           rdfs:subPropertyOf rico:isRelatedTo ;
                           rdfs:domain rico:Event ;
                           rdfs:comment """Connects an Event to a Thing that is associated with the
            existence and lifecycle of the Event."""@en ;
                           rdfs:isDefinedBy <https://www.ica.org/standards/RiC/ontology> ;
                           rdfs:label "is event associated with "@en ;
                           rico:RiCCMCorrespondingComponent """RiC-R057 ('is event associated with'
            relation)"""@en .


###  https://www.ica.org/standards/RiC/ontology#isInstantiationAssociatedWithInstantiation
rico:isInstantiationAssociatedWithInstantiation rdf:type owl:ObjectProperty ;
                                                rdfs:subPropertyOf rico:isRelatedTo ;
                                                rdf:type owl:SymmetricProperty ;
                                                rdfs:domain rico:Instantiation ;
                                                rdfs:range rico:Instantiation ;
                                                rdfs:comment """Connects two Instantiations. This object property is
            symmetric."""@en ;
                                                rdfs:isDefinedBy <https://www.ica.org/standards/RiC/ontology> ;
                                                rdfs:label "is instantiation associated with instantiation "@en ;
                                                rico:RiCCMCorrespondingComponent """RiC-R034 ('is instantiation associated with
            instantiation' relation)"""@en .


###  https://www.ica.org/standards/RiC/ontology#isInstantiationOf
rico:isInstantiationOf rdf:type owl:ObjectProperty ;
                       rdfs:subPropertyOf rico:isRelatedTo ;
                       rdfs:domain rico:Instantiation ;
                       rdfs:range rico:RecordResource ;
                       rdfs:comment "Inverse of 'has instantiation' object property."@en ;
                       rdfs:isDefinedBy <https://www.ica.org/standards/RiC/ontology> ;
                       rdfs:label "is instantiation of"@en ;
                       <http://www.w3.org/2004/02/skos/core#changeNote> [ ] ,
[ ] ;
rico:RiCCMCorrespondingComponent """RiC-R025i ('is instantiation of'
            relation)"""@en .


###  https://www.ica.org/standards/RiC/ontology#isOrWasCategoryOf
rico:isOrWasCategoryOf rdf:type owl:ObjectProperty ;
                       rdfs:subPropertyOf rico:isRelatedTo ;
                       rdfs:domain rico:Type ;
                       rdfs:range rico:Thing ;
                       rdfs:comment """Connects a Type (a category) to a Thing that it categorizes or
            categorized."""@en ;
                       rdfs:isDefinedBy <https://www.ica.org/standards/RiC/ontology> ;
                       rdfs:label "is or was category of"@en ;
                       <http://www.w3.org/2004/02/skos/core#changeNote> [ ] .


###  https://www.ica.org/standards/RiC/ontology#isOrWasContainedBy
rico:isOrWasContainedBy rdf:type owl:ObjectProperty ;
                        rdfs:subPropertyOf rico:isAssociatedWithPlace ,
                                           rico:isOrWasPartOf ,
                                           rico:isPlaceAssociatedWith ;
                        rdfs:domain rico:Place ;
                        rdfs:range rico:Place ;
                        rdfs:comment """Inverse of 'contains or contained' object
            property."""@en ;
                        rdfs:isDefinedBy <https://www.ica.org/standards/RiC/ontology> ;
                        rdfs:label "is or was contained by"@en ;
                        <http://www.w3.org/2004/02/skos/core#changeNote> [ ] ;
rico:RiCCMCorrespondingComponent """RiC-R007i ('is or was contained by'
            relation)"""@en .


###  https://www.ica.org/standards/RiC/ontology#isOrWasControllerOf
rico:isOrWasControllerOf rdf:type owl:ObjectProperty ;
                         rdfs:subPropertyOf rico:hasOrHadAuthorityOver ,
                                            rico:hasOrHadSubordinate ;
                         rdfs:domain rico:Agent ;
                         rdfs:range rico:Agent ;
                         rdfs:comment """Connects an Agent to another Agent it controls or controlled via
            Activities, i.e. controls by function."""@en ;
                         rdfs:isDefinedBy <https://www.ica.org/standards/RiC/ontology> ;
                         rdfs:label "is or was controller of"@en ;
                         <http://www.w3.org/2004/02/skos/core#changeNote> [ ] ;
rico:RiCCMCorrespondingComponent """RiC-R041 ('is or was controller of'
            relation)"""@en .


###  https://www.ica.org/standards/RiC/ontology#isOrWasIncludedIn
rico:isOrWasIncludedIn rdf:type owl:ObjectProperty ;
                       rdfs:subPropertyOf rico:isRecordResourceAssociatedWithRecordResource ;
                       rdfs:domain [ rdf:type owl:Class ;
                                     owl:unionOf ( rico:Record
                                                   rico:RecordSet
                                                 )
                                   ] ;
                       rdfs:range rico:RecordSet ;
                       rdfs:comment """Inverse of 'includes or included' object
            property."""@en ;
                       rdfs:isDefinedBy <https://www.ica.org/standards/RiC/ontology> ;
                       rdfs:label "is or was included in"@en ;
                       <http://www.w3.org/2004/02/skos/core#changeNote> [ ] ;
rico:RiCCMCorrespondingComponent """RiC-R024i ('is or was included in'
            relation)"""@en .


###  https://www.ica.org/standards/RiC/ontology#isOrWasLeaderOf
rico:isOrWasLeaderOf rdf:type owl:ObjectProperty ;
                     rdfs:subPropertyOf rico:isOrWasControllerOf ;
                     rdfs:domain rico:Person ;
                     rdfs:range rico:Group ;
                     rdfs:comment """Connects a Person to the Group that Person leads or led in the
            past."""@en ;
                     rdfs:isDefinedBy <https://www.ica.org/standards/RiC/ontology> ;
                     rdfs:label "is or was leader of"@en ;
                     <http://www.w3.org/2004/02/skos/core#changeNote> [ ] ;
rico:RiCCMCorrespondingComponent """RiC-R042 ('is or was leader of'
            relation)"""@en .


###  https://www.ica.org/standards/RiC/ontology#isOrWasMainSubjectOf
rico:isOrWasMainSubjectOf rdf:type owl:ObjectProperty ;
                          rdfs:subPropertyOf rico:isOrWasSubjectOf ;
                          rdfs:range rico:RecordResource ;
                          rdfs:label "is or was main subject of"@en .


###  https://www.ica.org/standards/RiC/ontology#isOrWasOwnerOf
rico:isOrWasOwnerOf rdf:type owl:ObjectProperty ;
                    rdfs:subPropertyOf rico:hasOrHadAuthorityOver ;
                    rdfs:comment """Connects a Group, Person or Position to a Thing that this Agent
            owns or owned."""@en ;
                    rdfs:isDefinedBy <https://www.ica.org/standards/RiC/ontology> ;
                    rdfs:label "is or was owner of"@en ;
                    <http://www.w3.org/2004/02/skos/core#changeNote> [ ] ;
rico:RiCCMCorrespondingComponent """RiC-R037 ('is or was owner of'
            relation)"""@en .


###  https://www.ica.org/standards/RiC/ontology#isOrWasPartOf
rico:isOrWasPartOf rdf:type owl:ObjectProperty ;
                   rdfs:subPropertyOf rico:isRelatedTo ;
                   rdfs:domain rico:Thing ;
                   rdfs:range rico:Thing ;
                   rdfs:comment "Inverse of 'has or had part' relation."@en ;
                   rdfs:isDefinedBy <https://www.ica.org/standards/RiC/ontology> ;
                   rdfs:label "is or was part of"@en ;
                   <http://www.w3.org/2004/02/skos/core#changeNote> [ ] ;
rico:RiCCMCorrespondingComponent """RiC-R002i (is or was part of
            relation)"""@en .


###  https://www.ica.org/standards/RiC/ontology#isOrWasParticipantIn
rico:isOrWasParticipantIn rdf:type owl:ObjectProperty ;
                          rdfs:subPropertyOf rico:isAssociatedWithEvent ;
                          rdfs:range rico:Event ;
                          rdfs:comment """Inverse of 'has or had participant' object
            property."""@en ;
                          rdfs:isDefinedBy <https://www.ica.org/standards/RiC/ontology> ;
                          rdfs:label "is or was participant in"@en ;
                          <http://www.w3.org/2004/02/skos/core#changeNote> [ ] ;
rico:RiCCMCorrespondingComponent """RiC-R058i ('is or was participant in'
            relation)"""@en .


###  https://www.ica.org/standards/RiC/ontology#isOrWasPerformedBy
rico:isOrWasPerformedBy rdf:type owl:ObjectProperty ;
                        rdfs:subPropertyOf rico:hasOrHadParticipant ;
                        owl:inverseOf rico:performsOrPerformed ;
                        rdfs:domain rico:Activity ;
                        rdfs:range rico:Agent ;
                        rdfs:comment """Connects an Activity to an Agent that performed or performs the
            Activity."""@en ;
                        rdfs:isDefinedBy <https://www.ica.org/standards/RiC/ontology> ;
                        rdfs:label "is or was performed by"@en ;
                        <http://www.w3.org/2004/02/skos/core#changeNote> [ ] ;
rico:RiCCMCorrespondingComponent """RiC-R060 ('is or was performed by'
            relation)"""@en .


###  https://www.ica.org/standards/RiC/ontology#isOrWasSubjectOf
rico:isOrWasSubjectOf rdf:type owl:ObjectProperty ;
                      rdfs:subPropertyOf rico:isRelatedTo ;
                      rdfs:range rico:RecordResource ;
                      rdfs:comment "Inverse of 'has or had subject' object property."@en ;
                      rdfs:label "is or was subject of"@en .


###  https://www.ica.org/standards/RiC/ontology#isOrWasUnderAuthorityOf
rico:isOrWasUnderAuthorityOf rdf:type owl:ObjectProperty ;
                             rdfs:subPropertyOf rico:isRelatedTo ;
                             rdfs:range rico:Agent ;
                             rdfs:comment """Inverse of 'has or had authority over' object
            property."""@en ;
                             rdfs:isDefinedBy <https://www.ica.org/standards/RiC/ontology> ;
                             rdfs:label "is or was under authority of"@en ;
                             <http://www.w3.org/2004/02/skos/core#changeNote> [ ] ;
rico:RiCCMCorrespondingComponent """RiC-R036i ('is or was under authority of'
            relation)"""@en .


###  https://www.ica.org/standards/RiC/ontology#isPlaceAssociatedWith
rico:isPlaceAssociatedWith rdf:type owl:ObjectProperty ;
                           rdfs:subPropertyOf rico:isRelatedTo ;
                           rdfs:domain rico:Place ;
                           rdfs:range rico:Thing ;
                           rdfs:comment """Connects a Place to a Thing that Place is associated with the
            existence and lifecycle of."""@en ;
                           rdfs:isDefinedBy <https://www.ica.org/standards/RiC/ontology> ;
                           rdfs:label "is place associated with "@en ;
                           rico:RiCCMCorrespondingComponent """RiC-R074 ('is place associated with'
            relation)"""@en .


###  https://www.ica.org/standards/RiC/ontology#isProvenanceOf
rico:isProvenanceOf rdf:type owl:ObjectProperty ;
                    rdfs:subPropertyOf rico:isRelatedTo ;
                    rdfs:domain rico:Agent ;
                    rdfs:range [ rdf:type owl:Class ;
                                 owl:unionOf ( rico:Instantiation
                                               rico:RecordResource
                                             )
                               ] ;
                    rdfs:comment "inverse of 'has provenance' object property."@en ;
                    rdfs:isDefinedBy <https://www.ica.org/standards/RiC/ontology> ;
                    rdfs:label "is provenance of "@en ;
                    rico:RiCCMCorrespondingComponent """RiC-R026i ('is provenance of'
            relation)"""@en .


###  https://www.ica.org/standards/RiC/ontology#isRecordResourceAssociatedWithRecordResource
rico:isRecordResourceAssociatedWithRecordResource rdf:type owl:ObjectProperty ;
                                                  rdfs:subPropertyOf rico:isRelatedTo ;
                                                  rdf:type owl:SymmetricProperty ;
                                                  rdfs:domain rico:RecordResource ;
                                                  rdfs:range rico:RecordResource ;
                                                  rdfs:label "is record resource associated with record resource"@en .


###  https://www.ica.org/standards/RiC/ontology#isRecordSetTypeOf
rico:isRecordSetTypeOf rdf:type owl:ObjectProperty ;
                       rdfs:subPropertyOf rico:isOrWasCategoryOf ;
                       rdfs:domain rico:RecordSetType ;
                       rdfs:range rico:RecordSet ;
                       rdfs:comment """Connects a Record Set Type to a Record Set that it
            categorizes."""@en ;
                       rdfs:isDefinedBy <https://www.ica.org/standards/RiC/ontology> ;
                       rdfs:label "is record set type of"@en ;
                       <http://www.w3.org/2004/02/skos/core#changeNote> [ ] .


###  https://www.ica.org/standards/RiC/ontology#isRelatedTo
rico:isRelatedTo rdf:type owl:ObjectProperty ,
                          owl:SymmetricProperty ;
                 rdfs:comment """The most generic object property. Connects an Thing to any other
            Thing This is a symmetric object property."""@en ;
                 rdfs:isDefinedBy <https://www.ica.org/standards/RiC/ontology> ;
                 rdfs:label "is related to "@en ;
                 rico:RiCCMCorrespondingComponent """RiC-R001 (is related to
            relation)"""@en .


###  https://www.ica.org/standards/RiC/ontology#isRepresentationTypeOf
rico:isRepresentationTypeOf rdf:type owl:ObjectProperty ;
                            rdfs:subPropertyOf rico:isOrWasCategoryOf ;
                            rdfs:domain rico:RepresentationType ;
                            rdfs:range rico:Instantiation ;
                            rdfs:comment """Connects a Representation Type to an Instantiation that it
            categorizes."""@en ;
                            rdfs:isDefinedBy <https://www.ica.org/standards/RiC/ontology> ;
                            rdfs:label "is representation type of"@en ;
                            <http://www.w3.org/2004/02/skos/core#changeNote> [ ] .


###  https://www.ica.org/standards/RiC/ontology#performsOrPerformed
rico:performsOrPerformed rdf:type owl:ObjectProperty ;
                         rdfs:subPropertyOf rico:isOrWasParticipantIn ;
                         rdfs:domain rico:Agent ;
                         rdfs:range rico:Activity ;
                         rdfs:comment """Inverse of 'is or was performed by' object
            property."""@en ;
                         rdfs:isDefinedBy <https://www.ica.org/standards/RiC/ontology> ;
                         rdfs:label "performs or performed"@en ;
                         <http://www.w3.org/2004/02/skos/core#changeNote> [ ] ;
rico:RiCCMCorrespondingComponent """RiC-R060i ('performs or performed'
            relation)"""@en .


###  https://www.ica.org/standards/RiC/ontology#precedesInTime
rico:precedesInTime rdf:type owl:ObjectProperty ;
                    rdfs:subPropertyOf rico:precedesOrPreceded .


###  https://www.ica.org/standards/RiC/ontology#precedesOrPreceded
rico:precedesOrPreceded rdf:type owl:ObjectProperty ;
                        rdfs:subPropertyOf rico:isRelatedTo ;
                        rdfs:comment """Connects a Thing to a Thing that follows or followed it in some
            sequence."""@en ;
                        rdfs:isDefinedBy <https://www.ica.org/standards/RiC/ontology> ;
                        rdfs:label "precedes or preceded"@en ;
                        <http://www.w3.org/2004/02/skos/core#changeNote> [ ] ;
<http://www.w3.org/2004/02/skos/core#scopeNote> """The relation does not specify by itself what criteria are used
            for ordering the sequence. There may actually be zero to many intermediate Entities,
            ignored or unkown, in the sequence between the two connected Things. Can be used, for
            example, for specifying that some Record 'precedes' (has next) some Record within a
            Record Set."""@en ;
rico:RiCCMCorrespondingComponent """RiC-R008 ('precedes or preceded'
            relation)"""@en .


###  https://www.ica.org/standards/RiC/ontology#resultsOrResultedFrom
rico:resultsOrResultedFrom rdf:type owl:ObjectProperty ;
                           rdfs:subPropertyOf rico:isAssociatedWithEvent ;
                           owl:inverseOf rico:resultsOrResultedIn ;
                           rdfs:range rico:Event ;
                           rdfs:comment """Inverse of 'results or resulted in' object
            property."""@en ;
                           rdfs:isDefinedBy <https://www.ica.org/standards/RiC/ontology> ;
                           rdfs:label "results or resulted from"@en ;
                           <http://www.w3.org/2004/02/skos/core#changeNote> [ ] ;
rico:RiCCMCorrespondingComponent """RiC-R061i ('results or resulted from'
            relation)"""@en .


###  https://www.ica.org/standards/RiC/ontology#resultsOrResultedIn
rico:resultsOrResultedIn rdf:type owl:ObjectProperty ;
                         rdfs:subPropertyOf rico:isEventAssociatedWith ;
                         rdfs:domain rico:Event ;
                         rdfs:comment """Connects an Event to a Thing that results or resulted from the
            Event."""@en ;
                         rdfs:isDefinedBy <https://www.ica.org/standards/RiC/ontology> ;
                         rdfs:label "results or resulted in"@en ;
                         <http://www.w3.org/2004/02/skos/core#changeNote> [ ] ;
rico:RiCCMCorrespondingComponent """RiC-R061 ('results or resulted in'
            relation)"""@en .


###  https://www.wikidata.org/wiki/Property:P106
wd:Property:P106 rdf:type owl:ObjectProperty ;
                 rdfs:label "occupation"@en .


###  https://www.wikidata.org/wiki/Property:P166
wd:Property:P166 rdf:type owl:ObjectProperty ;
                 rdfs:label "award received"@en .


###  https://www.wikidata.org/wiki/Property:P18
wd:Property:P18 rdf:type owl:ObjectProperty ;
                rdfs:label "image"@en .


###  https://www.wikidata.org/wiki/Property:P2031
wd:Property:P2031 rdf:type owl:ObjectProperty ;
                  rdfs:label "work period (start)"@en .


###  https://www.wikidata.org/wiki/Property:P31
wd:Property:P31 rdf:type owl:ObjectProperty ;
                rdfs:label "is instance of"@en .


###  https://www.wikidata.org/wiki/Property:P6715
wd:Property:P6715 rdf:type owl:ObjectProperty ;
                  rdfs:label "SIUSA archive creator person ID"@en .


###  https://www.wikidata.org/wiki/Property:P69
wd:Property:P69 rdf:type owl:ObjectProperty ;
                rdfs:label "educated at"@en .


###  https://www.wikidata.org/wiki/Property:P734
wd:Property:P734 rdf:type owl:ObjectProperty ;
                 rdfs:label "cognome"@it ,
                            "family name"@en .


###  https://www.wikidata.org/wiki/Property:P735
wd:Property:P735 rdf:type owl:ObjectProperty ;
                 rdfs:label "given name"@en .


###  https://www.wikidata.org/wiki/Property:P800
wd:Property:P800 rdf:type owl:ObjectProperty ;
                 rdfs:label "notable work"@en .


###  https://www.wikidata.org/wiki/Property:1066
<https://www.wikidata.org/wiki/Property:1066> rdf:type owl:ObjectProperty ;
                                              rdfs:label "student of"@en .


###  https://www.wikidata.org/wiki/Property:2032
<https://www.wikidata.org/wiki/Property:2032> rdf:type owl:ObjectProperty ;
                                              rdfs:label "work period (end)"@en .


###  https://www.wikidata.org/wiki/Property:26
<https://www.wikidata.org/wiki/Property:26> rdf:type owl:ObjectProperty ;
                                            rdfs:label "spouse"@en .


#################################################################
#    Data properties
#################################################################

###  https://dmikhaylova.github.io/itdt_ontology#exists
:exists rdf:type owl:DatatypeProperty ;
        rdfs:domain :ArchitecturalProject ;
        rdfs:range xsd:boolean ;
        rdfs:comment "Information about existence of the work carried out by an architectural project on the moment of the description."@en ;
        rdfs:label "exists"@en .


###  https://dmikhaylova.github.io/itdt_ontology#wasCarriedOut
:wasCarriedOut rdf:type owl:DatatypeProperty ;
               rdfs:domain :ArchitecturalProject ;
               rdfs:range xsd:boolean ;
               rdfs:comment "Information about whether an architectural project was carried out (e.g. the building was built, the restoration works were completed) or not."@en ;
               rdfs:label "was carried out"@en .


###  https://dmikhaylova.github.io/itdt_ontology/#arrangement
:arrangement rdf:type owl:DatatypeProperty ;
             rdfs:domain rico:RecordSet ;
             rdfs:range rdfs:Literal ;
             rdfs:comment "Information about the arrangement of records in a record set. Corresponds to the 3.4.1 of ISAD(G)."@en ;
             rdfs:label "arrangement"@en .


###  https://www.ica.org/standards/RiC/ontology#conditionsOfAccess
rico:conditionsOfAccess rdf:type owl:DatatypeProperty ;
                        rdfs:domain [ rdf:type owl:Class ;
                                      owl:unionOf ( rico:Instantiation
                                                    rico:RecordResource
                                                  )
                                    ] ;
                        rdfs:range rdfs:Literal ;
                        rdfs:comment """Terms and circumstances affecting the availability of a Record
            Resource for consultation. Such conditions may originate in laws, regulations and
            policies, including those pertaining to privacy and security concerns or restrictions;
            they may concern a specific Instantiation of a Record Resource, for example, conditions
            that require preservation treatment; or they may specify the software or hardware
            necessary to access the Instantiation."""@en ;
                        rdfs:isDefinedBy <https://www.ica.org/standards/RiC/ontology> ;
                        rdfs:label "conditions of access"@en ;
                        <http://www.w3.org/2004/02/skos/core#changeNote> [ ] ,
[ ] ;
<http://www.w3.org/2004/02/skos/core#example> """Acceso libre a través de los terminales de
            consulta"""@es ,
                                              """Recognita software, min. version 3.0, is needed in order to open
            the file."""@en ,
                                              "closed as awaiting conservation treatment"@en ,
                                              "closed under data protection legislation"@en ,
                                              "open"@en ,
                                              """the Archives cannot provide VHS reader to access the content of
            the tape."""@en ;
<http://www.w3.org/2004/02/skos/core#scopeNote> """This property provides information about the accessibility of
            a Record Resource, as well as the physical, technical or legal limitations that exist
            for providing access to it."""@en ;
rico:RiCCMCorrespondingComponent """Corresponds to RiC-A08 (Conditions of Access
            attribute)"""@en .


###  https://www.ica.org/standards/RiC/ontology#conditionsOfUse
rico:conditionsOfUse rdf:type owl:DatatypeProperty ;
                     rdfs:domain [ rdf:type owl:Class ;
                                   owl:unionOf ( rico:Instantiation
                                                 rico:RecordResource
                                               )
                                 ] ;
                     rdfs:range rdfs:Literal ;
                     rdfs:comment """Terms and circumstances affecting the use of a Record Resource
            after access has been provided. Includes conditions governing reproduction of the Record
            Resource under applicable copyright (intellectual property) and/or property legislation,
            and of the Instantiation, due to conservation status."""@en ;
                     rdfs:isDefinedBy <https://www.ica.org/standards/RiC/ontology> ;
                     rdfs:label "conditions of use"@en ;
                     <http://www.w3.org/2004/02/skos/core#changeNote> [ ] ,
[ ] ;
<http://www.w3.org/2004/02/skos/core#example> "Freely usable without restrictions"@en ,
                                              """The permission of the owner of the Record must be obtained
            before use."""@en ,
                                              """The record cannot be copied using warm light copying machines or
            photographed using flashlight."""@en ;
rico:RiCCMCorrespondingComponent """Corresponds to RiC-A09 (Conditions of Use
            attribute)"""@en .


###  https://www.ica.org/standards/RiC/ontology#descriptiveNote
rico:descriptiveNote rdf:type owl:DatatypeProperty ;
                     rdfs:range rdfs:Literal ;
                     rdfs:comment """Descriptive information about an entity that is not otherwise
            addressed."""@en ;
                     rdfs:isDefinedBy <https://www.ica.org/standards/RiC/ontology> ;
                     rdfs:label "descriptive note"@en ;
                     rico:RiCCMCorrespondingComponent """Corresponds to RiC-A16 (Descriptive Note
            attribute)"""@en .


###  https://www.ica.org/standards/RiC/ontology#history
rico:history rdf:type owl:DatatypeProperty ;
             rdfs:domain [ rdf:type owl:Class ;
                           owl:unionOf ( rico:Activity
                                         rico:Agent
                                         rico:Event
                                         rico:Instantiation
                                         rico:Place
                                         rico:RecordResource
                                         rico:Rule
                                       )
                         ] ;
             rdfs:range rdfs:Literal ;
             rdfs:comment """Summary of the development of an entity, since its origin until
            present time."""@en ;
             rdfs:isDefinedBy <https://www.ica.org/standards/RiC/ontology> ;
             rdfs:label "history"@en ;
             <http://www.w3.org/2004/02/skos/core#changeNote> [ ] ;
<http://www.w3.org/2004/02/skos/core#example> """El primer sorteo de lotería se celebró el 13 de mayo de 1771,
            siendo desarrollado por la Real Lotería General de Nueva España…
            (Activity)"""@es ,
                                              """Nacido en Barbastro en 1892, donde realizó sus primeros estudios
            con los escolapios. Licenciado en Derecho por la Universidad de Zaragoza, aprobó las
            oposiciones al cuerpo nacional de notarios…(Person)"""@es ,
                                              """The manuscripts are part of the collections of Robert Harley (d
            1724) and Edward Harley (d 1741), 1st and 2nd Earls of Oxford, that were brought by
            Parliament and transferred to the British Museum in 1753. Those materials were then
            separated into this collection and those for Harley Charters and Harley Rolls and became
            part of the collections of the British Library in 1972. (Record Set)"""@en ;
<http://www.w3.org/2004/02/skos/core#scopeNote> """History can alternatively be represented by a series of
            related Events."""@en ;
rico:RiCCMCorrespondingComponent """Corresponds to RiC-A21 (History
            attribute)"""@en .


###  https://www.ica.org/standards/RiC/ontology#identifier
rico:identifier rdf:type owl:DatatypeProperty ;
                rdfs:domain rico:Thing ;
                rdfs:range rdfs:Literal ;
                rdfs:comment """A word, number, letter, symbol, or any combination of these used
            to uniquely identify or reference an individual instance of an entity within a specific
            information domain. Includes Global Persistent Identifiers (globally unique and
            persistently resolvable identifier for the entity) and/or Local
            Identifiers."""@en ;
                rdfs:isDefinedBy <https://www.ica.org/standards/RiC/ontology> ;
                rdfs:label "identifier"@en ;
                <http://www.w3.org/2004/02/skos/core#changeNote> [ ] ,
[ ] ;
<http://www.w3.org/2004/02/skos/core#example> "Ark ID: w6tz44ht"@en ,
                                              """BUD-01-F002 [example of a classification number from a corporate
            file plan]"""@en ,
                                              """F 1204 [example of a local identifier for a Record Set assigned
            by a repository]"""@en ,
                                              "ISNI : 0000000073572182"@en ,
                                              """NAS1/A/1.1 [example of local identifier for a
            Record]"""@en ,
                                              "SNAC ID: 83847206"@en ;
<http://www.w3.org/2004/02/skos/core#scopeNote> """Use only if you don't use Identifier class for handling
            identifiers. Within a given domain (a closed system), identifiers are used to uniquely
            reference instances of an entity. Identifiers are instruments of control that facilitate
            management of the entities within the domain. The formulation of identifiers commonly is
            based on rules."""@en ;
rico:RiCCMCorrespondingComponent """Corresponds to RiC-A22 (Identifier
            attribute)"""@en .


###  https://www.ica.org/standards/RiC/ontology#instantiationExtent
rico:instantiationExtent rdf:type owl:DatatypeProperty ;
                         rdfs:subPropertyOf rico:physicalOrLogicalExtent ;
                         rdfs:domain rico:Instantiation ;
                         rdfs:range rdfs:Literal ;
                         rdfs:comment """Countable characteristics of the Instantiation expressed as a
            quantity."""@en ;
                         rdfs:isDefinedBy <https://www.ica.org/standards/RiC/ontology> ;
                         rdfs:label "Instantiation extent"@en ;
                         <http://www.w3.org/2004/02/skos/core#changeNote> [ ] ;
<http://www.w3.org/2004/02/skos/core#example> "Size of PDF-file: 1.5 MB"@en ,
                                              "The book register has 345 written leaves."@en ;
<http://www.w3.org/2004/02/skos/core#scopeNote> """For a given Record Resource, the Instantiation Extent may
            vary, based on format, density of information on the carrier, etc. For example, a file
            of 1500 words (Record Resource Extent) may have Instantiation Extent 3kb as a Word
            document and 5kb as a PDF file, and instantiations may be represented on a CD of 700mb
            (Carrier Extent). Use if you don't use InstantiationExtent class and its properties for
            handling such information."""@en ;
rico:RiCCMCorrespondingComponent """Corresponds to RiC-A23 (Instantiation Extent
            attribute)"""@en .


###  https://www.ica.org/standards/RiC/ontology#instantiationStructure
rico:instantiationStructure rdf:type owl:DatatypeProperty ;
                            rdfs:subPropertyOf rico:structure ;
                            rdfs:domain rico:Instantiation ;
                            rdfs:range rdfs:Literal ;
                            rdfs:comment """Information about the physical arrangement and composition of an
            Instantiation."""@en ;
                            rdfs:isDefinedBy <https://www.ica.org/standards/RiC/ontology> ;
                            rdfs:label "Instantiation structure"@en ;
                            <http://www.w3.org/2004/02/skos/core#changeNote> [ ] ;
rico:RiCCMCorrespondingComponent """Specialization of RiC-A40 (Structure
            attribute)"""@en .


###  https://www.ica.org/standards/RiC/ontology#name
rico:name rdf:type owl:DatatypeProperty ;
          rdfs:domain rico:Thing ;
          rdfs:range rdfs:Literal ;
          rdfs:comment """A label, title or term designating the entity in order to make
            it distinguishable from other similar entities. For Record Resource or Instantiation,
            the Name is generally assigned by an Agent as most do not have a Name given when
            created."""@en ;
          rdfs:isDefinedBy <https://www.ica.org/standards/RiC/ontology> ;
          rdfs:label "name"@en ;
          <http://www.w3.org/2004/02/skos/core#changeNote> [ ] ;
<http://www.w3.org/2004/02/skos/core#example> "4 March 1842"@en ,
                                              """Digital copy of the Pomarius archival inventory from
            1575"""@en ,
                                              "Nelson Mandela"@en ,
                                              "Papers of the Earls of Liverpool"@en ,
                                              "Sketch Map of the Qatar Peninsula"@en ,
                                              """The Letter of Neacsu from Campulung to the Mayor of
            Brasov"""@en ,
                                              "fundraising, University of Glasgow"@en ,
                                              "hearing services"@en ;
<http://www.w3.org/2004/02/skos/core#scopeNote> """Use only if you don't use Name class for handling
            names."""@en ;
rico:RiCCMCorrespondingComponent """Corrresponds to RiC-A28 (Name
            attribute)"""@en .


###  https://www.ica.org/standards/RiC/ontology#physicalOrLogicalExtent
rico:physicalOrLogicalExtent rdf:type owl:DatatypeProperty ;
                             rdfs:domain [ rdf:type owl:Class ;
                                           owl:unionOf ( rico:Instantiation
                                                         rico:RecordResource
                                                       )
                                         ] ;
                             rdfs:range rdfs:Literal ;
                             rdfs:comment """Countable characteristics of the content of an entity expressed
            as a quantity."""@en ;
                             rdfs:isDefinedBy <https://www.ica.org/standards/RiC/ontology> ;
                             rdfs:label "physical or logical extent"@en ;
                             <http://www.w3.org/2004/02/skos/core#scopeNote> """Provided for usability reasons. Use only if you cannot use the
            subproperties (particularly if the same free text is being used in your current metadata
            for describing the record resource, carrier and instantiation extent)."""@en .


###  https://www.ica.org/standards/RiC/ontology#recordResourceExtent
rico:recordResourceExtent rdf:type owl:DatatypeProperty ;
                          rdfs:subPropertyOf rico:physicalOrLogicalExtent ;
                          rdfs:domain rico:RecordResource ;
                          rdfs:range rdfs:Literal ;
                          rdfs:comment """The quantity of information content as human experienced
            represented in the Record Resource. The method and precision of expressing the quantity
            of information represented in a Record Resource will vary by the kind of Record Resource
            being described as well as by processing economy constraints. For record sets, quantity
            may be expressed as number of records, or, for analogue records in particular, by the
            physical storage dimensions of the Record members. For individual records or record
            parts, quantity may be expressed in more precise terms. Use if you don't use
            RecordResourceExtent class and its properties for handling such
            information."""@en ;
                          rdfs:isDefinedBy <https://www.ica.org/standards/RiC/ontology> ;
                          rdfs:label "Record Resource extent"@en ;
                          <http://www.w3.org/2004/02/skos/core#changeNote> [ ] ,
[ ] ,
[ ] ,
[ ] ;
<http://www.w3.org/2004/02/skos/core#example> "1,500 words"@en ,
                                              "2 films"@en ,
                                              "2.065.735 characters"@en ,
                                              "3 minutes and 24 seconds"@en ,
                                              "34 poems"@en ,
                                              "6 maps"@en ,
                                              "6 photographs"@en ;
<http://www.w3.org/2004/02/skos/core#scopeNote> """The number, size or duration of the information content
            unit(s) remains the same even if the information is instantiated in various carriers.
            For example, a file of 1500 words (Record Resource Extent) may have Instantiation Extent
            3kb as a Word document and 5kb as a PDF file, and instantiations may be represented on a
            CD of 700mb (Carrier Extent). Use if you don't use RecordResourceExtent class and its
            properties for handling such information."""@en ;
rico:RiCCMCorrespondingComponent """Corresponds to RiC-A35 (Record Resource extent
            attribute)"""@en .


###  https://www.ica.org/standards/RiC/ontology#recordResourceStructure
rico:recordResourceStructure rdf:type owl:DatatypeProperty ;
                             rdfs:subPropertyOf rico:structure ;
                             rdfs:domain rico:RecordResource ;
                             rdfs:range rdfs:Literal ;
                             rdfs:comment """Information about the intellectual arrangement and composition
            of a Record Resource. For Record and Record Part, it encompasses information about the
            intellectual composition of the record, the presence of record parts and their
            functions. For Record Set, it encompasses information about the methodology or criteria
            used for arranging the Record Set members or Record members within the containing Record
            Set"""@en ;
                             rdfs:isDefinedBy <https://www.ica.org/standards/RiC/ontology> ;
                             rdfs:label "Record Resource structure"@en ;
                             <http://www.w3.org/2004/02/skos/core#changeNote> [ ] ;
<http://www.w3.org/2004/02/skos/core#example> """Inside each file, the records are arranged
            chronologically."""@en ,
                                              """The database has 3 related tables: names, addresses, and
            passport numbers."""@en ,
                                              """The record has 2 appendixes, comprising a full account of the
            income from car taxes and real estate taxes."""@en ,
                                              """The series have the files arranged according to the alphabetical
            order of the places concerned."""@en ;
rico:RiCCMCorrespondingComponent """Specialization of RiC-A40 (Structure
            attribute)"""@en .


###  https://www.ica.org/standards/RiC/ontology#scopeAndContent
rico:scopeAndContent rdf:type owl:DatatypeProperty ;
                     rdfs:domain rico:RecordResource ;
                     rdfs:range rdfs:Literal ;
                     rdfs:comment """Summary of the scope (such as time periods, geography) and
            content (such as subject matter, administrative processes) of the Record Resource. It
            should highlight the information conveyed in the Record Resource, why it was created,
            received, and/or maintained, and the Agents connected to it. Scope and Content provides
            a more complete summary of the informational content of the Record Resource. It may
            include description of relations with agents, activities, dates and places, or with
            other record resources. It is not to be confused with the History attribute which
            focuses on the origination and subsequence changes to a Record Resource."""@en ;
                     rdfs:isDefinedBy <https://www.ica.org/standards/RiC/ontology> ;
                     rdfs:label "scope and content"@en ;
                     <http://www.w3.org/2004/02/skos/core#changeNote> [ ] ,
[ ] ;
<http://www.w3.org/2004/02/skos/core#example> "Among the witnesses, the duke of Normandy."@en ,
                                              """Includes a detailed list of the lands and villages given by the
            King to the Abbey."""@en ,
                                              """Letter from Vlad the Impaler (Dracula) to the Council of
            Kronstadt asking them to send military support against the Ottomans, within the
            framework of their alliance treaty."""@en ,
                                              """Se hace referencia a construcción del Gran Hotel, iniciada en
            1899 bajo el nombre de Casa Celestino. Tras su interrupción en 1902, continuó la obra ya
            con su nombre actual."""@es ,
                                              """The author explains why he does not agree with the decision made
            and adds that it cannot be applied."""@en ;
rico:RiCCMCorrespondingComponent """Corresponds to RiC-A38 (Scope and Content
            attribute)"""@en .


###  https://www.ica.org/standards/RiC/ontology#structure
rico:structure rdf:type owl:DatatypeProperty ;
               rdfs:domain [ rdf:type owl:Class ;
                             owl:unionOf ( rico:Instantiation
                                           rico:RecordResource
                                         )
                           ] ;
               rdfs:range rdfs:Literal ;
               rdfs:comment """Information about the intellectual arrangement and composition
            of a Record Resource or the physical arrangement and composition of an Instantiation.
            For Record and Record Part, it encompasses information about the intellectual
            composition of the record, the presence of record parts and their functions. For Record
            Set, it encompasses information about the methodology or criteria used for arranging the
            Record Set members or Record members within the containing Record Set. For
            Instantiation, it may comprise information about the composition of the physical
            elements of the instantiation"""@en ;
               rdfs:isDefinedBy <https://www.ica.org/standards/RiC/ontology> ;
               rdfs:label "structure"@en ;
               <http://www.w3.org/2004/02/skos/core#changeNote> [ ] ;
<http://www.w3.org/2004/02/skos/core#scopeNote> """Use only if you cannot use the subproperties (particularly if
            the same free text is being used in your current metadata for describing the record
            resource and the instantiation structure)."""@en ;
rico:RiCCMCorrespondingComponent """Corresponds to RiC-A40 (Structure
            attribute)"""@en .


###  https://www.ica.org/standards/RiC/ontology#title
rico:title rdf:type owl:DatatypeProperty ;
           rdfs:subPropertyOf rico:name ;
           rdfs:domain [ rdf:type owl:Class ;
                         owl:unionOf ( rico:Instantiation
                                       rico:RecordResource
                                       rico:Rule
                                     )
                       ] ;
           rdfs:range rdfs:Literal ;
           rdfs:comment """An identifying name of a Record Resource, Instantiation or
            Rule."""@en ;
           rdfs:isDefinedBy <https://www.ica.org/standards/RiC/ontology> ;
           rdfs:label "title"@en ;
           <http://www.w3.org/2004/02/skos/core#scopeNote> """Use only if you don't use Title class for handling
            titles."""@en ;
           rico:RiCCMCorrespondingComponent """Specialization of RiC-A28 (Name
            attribute)"""@en .


#################################################################
#    Classes
#################################################################

###  http://www.w3.org/2004/02/skos/core#Concept
<http://www.w3.org/2004/02/skos/core#Concept> rdf:type owl:Class .


###  http://www.w3.org/2004/02/skos/core#ConceptScheme
<http://www.w3.org/2004/02/skos/core#ConceptScheme> rdf:type owl:Class .


###  https://dmikhaylova.github.io/itdt_ontology/#AcceptancePhase
:AcceptancePhase rdf:type owl:Class ;
                 rdfs:subClassOf :ProjectPhase ;
                 rdfs:comment "The fourth phase of the project  that marks the end of construction works during which the building is accepted by an architect and then by a client."@en ;
                 rdfs:label "Acceptance Phase"@en .


###  https://dmikhaylova.github.io/itdt_ontology/#AnalysisPhase
:AnalysisPhase rdf:type owl:Class ;
               rdfs:subClassOf :ProjectPhase ;
               rdfs:comment "The first phase of the project during which an architect analyses the requirements (the laws and regulations to respect), the material conditions (the budget, building materials and techniques) and the construction site (the natural or urban context) for the future project:"@en ;
               rdfs:label "Analysis Phase"@en .


###  https://dmikhaylova.github.io/itdt_ontology/#ArchitecturalDrawing
:ArchitecturalDrawing rdf:type owl:Class ;
                      rdfs:subClassOf :GraphicalRecord ;
                      rdfs:comment "A drawing for architectural project or a drawing of architecture"@en ;
                      rdfs:label "Architectural Drawing"@en .


###  https://dmikhaylova.github.io/itdt_ontology/#ArchitecturalPhotograph
:ArchitecturalPhotograph rdf:type owl:Class ;
                         rdfs:subClassOf :GraphicalRecord ;
                         rdfs:comment "Architectural record that uses photography as a principal documentary form, photographs that have architecture as a main subject."@en ;
                         rdfs:label "Architectural Photograph"@en .


###  https://dmikhaylova.github.io/itdt_ontology/#ArchitecturalProject
:ArchitecturalProject rdf:type owl:Class ;
                      rdfs:subClassOf rico:Activity ,
                                      [ rdf:type owl:Restriction ;
                                        owl:onProperty :isCommissionedBy ;
                                        owl:allValuesFrom rico:Agent
                                      ] ,
                                      [ rdf:type owl:Restriction ;
                                        owl:onProperty :hasOrHadProjectPhase ;
                                        owl:minQualifiedCardinality "1"^^xsd:nonNegativeInteger ;
                                        owl:onClass :ProjectPhase
                                      ] ;
                      rdfs:comment "Artistic concepts comprising proposed undertakings or creations in architecture, or for the actual carrying out of such proposals. An activity carried out to design and/or construct a building."@en ;
                      rdfs:isDefinedBy "https://dmikhaylova.github.io/itdt_ontology"@en ;
                      rdfs:label "Architectural Project"@en .


###  https://dmikhaylova.github.io/itdt_ontology/#ArchitecturalRecord
:ArchitecturalRecord rdf:type owl:Class ;
                     rdfs:subClassOf rico:Record ;
                     rdfs:comment "A record that documents creative and project activity of an architect or an architect firm."@en ;
                     rdfs:label "Architectural Record"@en .


###  https://dmikhaylova.github.io/itdt_ontology/#Article
:Article rdf:type owl:Class ;
         rdfs:subClassOf :WrittenRecord ;
         rdfs:comment "Literary composition prepared for publication as an independent portion of a magazine or newspaper"@en ;
         rdfs:label "Article"@en .


###  https://dmikhaylova.github.io/itdt_ontology/#BidPhase
:BidPhase rdf:type owl:Class ;
          rdfs:subClassOf :ExecutionPhase ;
          rdfs:comment "The second stage of the execution phase of the project that has a goal to choose contractors and suppliers."@en ;
          rdfs:label "Bid Stage"@en .


###  https://dmikhaylova.github.io/itdt_ontology/#CarpentryPlan
:CarpentryPlan rdf:type owl:Class ;
               rdfs:subClassOf :ConstructionDrawing ;
               rdfs:comment "Drawing that illustrates door and windows frames and fixtures for a building."@en ;
               rdfs:label "Carpentry Plan"@en .


###  https://dmikhaylova.github.io/itdt_ontology/#ConceptualDrawing
:ConceptualDrawing rdf:type owl:Class ;
                   rdfs:subClassOf :ArchitecturalDrawing ;
                   rdfs:comment "Small-scale, free-hand drawings which give an idea of the design of the building project or express forms of the building project in symbolic way"@en ;
                   rdfs:label "Conceptual Drawing"@en .


###  https://dmikhaylova.github.io/itdt_ontology/#ConciseIdeaStage
:ConciseIdeaStage rdf:type owl:Class ;
                  rdfs:subClassOf :CreativePhase ;
                  rdfs:comment "The second stage of the creative phase during which an architect formulates a concise idea of the future building starting from a primary solid, a composition of spaces, an analogy or a metonymy and develops the idea from general vision to particular details, or vice versa .  During this stage, architects decide a formal typology of the future building. The documents and drawings resulting from this stage are conceptual and design drawings and are often equal to the papers submitted for design competition."@en ;
                  rdfs:label "Concise Idea Stage"@en .


###  https://dmikhaylova.github.io/itdt_ontology/#ConstructionDrawing
:ConstructionDrawing rdf:type owl:Class ;
                     rdfs:subClassOf :ArchitecturalDrawing ;
                     rdfs:comment "Drawing that is used to communicate information about buildings, specifically the mechanics of their construction, and used by the team tasked with erecting an edifice."@en ;
                     rdfs:label "Construction Drawing"@en .


###  https://dmikhaylova.github.io/itdt_ontology/#ConstructionPhase
:ConstructionPhase rdf:type owl:Class ;
                   rdfs:subClassOf :ExecutionPhase ;
                   rdfs:comment "The third and the last stage of the execution phase that has a goal to construct the designed building or to complete other works."@en ;
                   rdfs:label "Construction Stage"@en .


###  https://dmikhaylova.github.io/itdt_ontology/#ContextPhotograph
:ContextPhotograph rdf:type owl:Class ;
                   rdfs:subClassOf :ArchitecturalPhotograph ;
                   rdfs:comment "Photograph  that is taken by an architect in the stage of conceptual design or after the submission of the work and may include depictions of the construction site or surroundings."@en ;
                   rdfs:label "Context Photograph"@en .


###  https://dmikhaylova.github.io/itdt_ontology/#CreativePhase
:CreativePhase rdf:type owl:Class ;
               rdfs:subClassOf :ProjectPhase ;
               rdfs:comment "The second phase of the project during which an architect conceives and develops an idea for future building."@en ;
               rdfs:label "Creative Phase"@en .


###  https://dmikhaylova.github.io/itdt_ontology/#DesignDrawing
:DesignDrawing rdf:type owl:Class ;
               rdfs:subClassOf :ArchitecturalDrawing ;
               rdfs:comment "Drawings that refine conceptual drawings and are usually prepared using instruments"@en ;
               rdfs:label "Design Drawing"@en .


###  https://dmikhaylova.github.io/itdt_ontology/#DetailPhotograph
:DetailPhotograph rdf:type owl:Class ;
                  rdfs:subClassOf :ArchitecturalPhotograph ;
                  rdfs:comment "Photograph that depicts external or internal decorations of the building or particular construction solutions, usually shot with close-up."@en ;
                  rdfs:label "Detail Photograph"@en .


###  https://dmikhaylova.github.io/itdt_ontology/#DevelopmentStage
:DevelopmentStage rdf:type owl:Class ;
                  rdfs:subClassOf :CreativePhase ;
                  rdfs:comment "The final stage of the creative phase during which the concise idea evolves into a morphological scheme, where the quantity of necessary spaces is defined along with their elementary shape, position and relative size. The architect develops a scheme of spaces and volumes and produces consistent floor plans, sections, elevations and three-dimensional drawings. In this stage, an architect also produces drawings that verify geometrical consistency of the project."@en ;
                  rdfs:label "Development Stage"@en .


###  https://dmikhaylova.github.io/itdt_ontology/#Elevation
:Elevation rdf:type owl:Class ;
           rdfs:subClassOf :WorkingDrawing ;
           rdfs:comment "Drawing or work in another medium showing the arrangement of vertical elements of a building, either exterior or interior, as a direct projection to a vertical plane."@en ;
           rdfs:label "Elevation"@en .


###  https://dmikhaylova.github.io/itdt_ontology/#ExecutionPhase
:ExecutionPhase rdf:type owl:Class ;
                rdfs:subClassOf :ProjectPhase ;
                rdfs:comment "The third phase of the architectural project that has a goal to construct the designed building or to carry out other architectural work defined during the previous phase."@en ;
                rdfs:label "Execution Phase"@en .


###  https://dmikhaylova.github.io/itdt_ontology/#ExteriorPhotograph
:ExteriorPhotograph rdf:type owl:Class ;
                    rdfs:subClassOf :ArchitecturalPhotograph ;
                    rdfs:comment "Photograph that communicates the distribution of spaces of a building visible from outside."@en ;
                    rdfs:label "Exterior Photograph"@en .


###  https://dmikhaylova.github.io/itdt_ontology/#FloorPlan
:FloorPlan rdf:type owl:Class ;
           rdfs:subClassOf :WorkingDrawing ;
           rdfs:comment "Drawing or work in another two-dimensional medium that represent a horizontal section through a building taken above a floor to diagrammatically illustrate the enclosing walls, interior spaces, doors, and windows of a building."@en ;
           rdfs:label "Floor Plan"@en .


###  https://dmikhaylova.github.io/itdt_ontology/#FollowUpPhase
:FollowUpPhase rdf:type owl:Class ;
               rdfs:subClassOf :ProjectPhase ;
               rdfs:comment "The last phase of architectural project, often delayed indefinitely in time, that may include further interventions by an architect in the life of artefact, such as consultation for any problems, decorative works, renovations, communication with media, owners of the building and administrative offices."@en ;
               rdfs:label "Follow-up Phase"@en .


###  https://dmikhaylova.github.io/itdt_ontology/#FormalBuildingType
:FormalBuildingType rdf:type owl:Class ;
                    rdfs:subClassOf rico:Type ;
                    rdfs:comment "Categorization of the architectural project with respect to model of formal characteristics and organisation of internal spaces of the building that is meant to be designed and developed by the project."@en ;
                    rdfs:isDefinedBy "https://dmikhaylova.github.io/itdt_ontology"@en ;
                    rdfs:label "Formal Building Type"@en ;
                    <http://www.w3.org/2004/02/skos/core#example> "casa a ballatoio"@it ,
                                                                  "courtyard house"@en ,
                                                                  "roman theater"@en .


###  https://dmikhaylova.github.io/itdt_ontology/#FoundationPlan
:FoundationPlan rdf:type owl:Class ;
                rdfs:subClassOf :ConstructionDrawing ;
                rdfs:comment "Plan that illustrate the configuration and location of the foundation, which comprises the supporting elements of a building, located primarily below ground level, that transmit building loads to the soil or rock underneath."@en ;
                rdfs:label "Foundation Plan"@en .


###  https://dmikhaylova.github.io/itdt_ontology/#FunctionalBuildingType
:FunctionalBuildingType rdf:type owl:Class ;
                        rdfs:subClassOf rico:Type ,
                                        [ rdf:type owl:Restriction ;
                                          owl:onProperty :isFunctionalBuildingTypeOf ;
                                          owl:allValuesFrom :ArchitecturalProject
                                        ] ;
                        rdfs:comment "Categorization of the architectural project with respect to the intended function or use of the building that the project designs and develops."@en ;
                        rdfs:isDefinedBy "https://dmikhaylova.github.io/itdt_ontology"@en ;
                        rdfs:label "Functional Building Type"@en ;
                        <http://www.w3.org/2004/02/skos/core#example> "edificio per culto"@it ,
                                                                      "school building"@en .


###  https://dmikhaylova.github.io/itdt_ontology/#FurniturePlan
:FurniturePlan rdf:type owl:Class ;
               rdfs:subClassOf :ConstructionDrawing ;
               rdfs:comment "Drawing that indicates the precise location of each piece of furnishing for internal space of a building."@en ;
               rdfs:label "Furniture Plan"@en .


###  https://dmikhaylova.github.io/itdt_ontology/#GeneralPlan
:GeneralPlan rdf:type owl:Class ;
             rdfs:subClassOf :WorkingDrawing ;
             rdfs:comment "Overall plan, usually graphic and drawn on a small scale, into which the details of other specific plans are fitted."@en ;
             rdfs:label "General Plan"@en .


###  https://dmikhaylova.github.io/itdt_ontology/#GraphicalRecord
:GraphicalRecord rdf:type owl:Class ;
                 rdfs:subClassOf :ArchitecturalRecord ;
                 rdfs:comment "A document that contains images or designs created in the process of designing or constructing an architectural project."@en ;
                 rdfs:label "Graphical record"@en .


###  https://dmikhaylova.github.io/itdt_ontology/#InteriorDesignPlan
:InteriorDesignPlan rdf:type owl:Class ;
                    rdfs:subClassOf :ConstructionDrawing ;
                    rdfs:comment "Plan that describes the design of interiors of homes or other buildings, including placement of furniture, accessories, aesthetic or decorative schemes, and spatial arrangements."@en ;
                    rdfs:label "Interior Design Plan"@en .


###  https://dmikhaylova.github.io/itdt_ontology/#InteriorPhotograph
:InteriorPhotograph rdf:type owl:Class ;
                    rdfs:subClassOf :ArchitecturalPhotograph ;
                    rdfs:comment "Photograph that depicts the internal volumes distribution o a building or a room, interior design and furniture."@en ;
                    rdfs:label "Interior Photograph"@en .


###  https://dmikhaylova.github.io/itdt_ontology/#InteriorSystemsPlan
:InteriorSystemsPlan rdf:type owl:Class ;
                     rdfs:subClassOf :ConstructionDrawing ;
                     rdfs:comment "Drawings or works in another medium, often made by an engineer, that indicate the location of utilities, including water supply lines, fire hydrants, sewage disposal lines, and other utilities. As part of the construction process, these plans are generally required for submission to local authorities."@en ;
                     rdfs:label "Interior Systems Plan"@en .


###  https://dmikhaylova.github.io/itdt_ontology/#Invitation
:Invitation rdf:type owl:Class ;
            rdfs:subClassOf :WrittenRecord ;
            rdfs:comment "Printed or written expression requesting a person's company at a certain event at a given time and place."@en ;
            rdfs:label "Invitation"@en .


###  https://dmikhaylova.github.io/itdt_ontology/#Letter
:Letter rdf:type owl:Class ;
        rdfs:subClassOf :WrittenRecord ;
        rdfs:comment "Pieces of correspondence, sent and delivered."@en ;
        rdfs:label "Letter"@en .


###  https://dmikhaylova.github.io/itdt_ontology/#Model
:Model rdf:type owl:Class ;
       rdfs:subClassOf :ArchitecturalRecord ;
       rdfs:comment "Architectural record  that visualises architectural projects in three dimensions, often including a representation of the surrounding site or context."@en ;
       rdfs:label "Model"@en .


###  https://dmikhaylova.github.io/itdt_ontology/#PermitStage
:PermitStage rdf:type owl:Class ;
             rdfs:subClassOf :ExecutionPhase ;
             rdfs:comment "The first stage of the executive phase during which an architect develops further the idea and prepares a set of drawings and written documents to receive building permit."@en ;
             rdfs:label "Permit Stage"@en .


###  https://dmikhaylova.github.io/itdt_ontology/#PhysicalModel
:PhysicalModel rdf:type owl:Class ;
               rdfs:subClassOf :Model ;
               rdfs:comment "Architectural model in physical form."@en ;
               rdfs:label "Physical Model"@en .


###  https://dmikhaylova.github.io/itdt_ontology/#PresentationDrawing
:PresentationDrawing rdf:type owl:Class ;
                     rdfs:subClassOf :ArchitecturalDrawing ;
                     rdfs:comment "Drawings that imagine the appearance of the complete project and are prepared with shading, color, and perspective to win the client's approval, they often suggest vegetation, people and vehicles to bring image to life"@en ;
                     rdfs:label "Rendering"@en .


###  https://dmikhaylova.github.io/itdt_ontology/#ProcessPhotograph
:ProcessPhotograph rdf:type owl:Class ;
                   rdfs:subClassOf :ArchitecturalPhotograph ;
                   rdfs:comment "Photograph that depicts demolition or construction works of a building and taken to document internal structures of the building or to accompany the intermediate report of the construction works."@en ;
                   rdfs:label "Process Photograph"@en .


###  https://dmikhaylova.github.io/itdt_ontology/#ProjectParticipation
:ProjectParticipation rdf:type owl:Class ;
                      rdfs:subClassOf rico:Event ,
                                      [ rdf:type owl:Restriction ;
                                        owl:onProperty :hasOrHadProjectRole ;
                                        owl:maxQualifiedCardinality "1"^^xsd:nonNegativeInteger ;
                                        owl:onClass :ProjectRole
                                      ] ,
                                      [ rdf:type owl:Restriction ;
                                        owl:onProperty :isOrWasProjectParticipationOf ;
                                        owl:maxQualifiedCardinality "1"^^xsd:nonNegativeInteger ;
                                        owl:onClass [ rdf:type owl:Class ;
                                                      owl:unionOf ( :ArchitecturalProject
                                                                    :ProjectPhase
                                                                  )
                                                    ]
                                      ] ,
                                      [ rdf:type owl:Restriction ;
                                        owl:onProperty rico:hasOrHadParticipant ;
                                        owl:maxQualifiedCardinality "1"^^xsd:nonNegativeInteger ;
                                        owl:onClass rico:Agent
                                      ] ;
                      rdfs:comment "This class creates ternary relation between Agent and Project, that they participate in with some particular Project role"@en ;
                      rdfs:label "Project Participation"@en .


###  https://dmikhaylova.github.io/itdt_ontology/#ProjectPhase
:ProjectPhase rdf:type owl:Class ;
              rdfs:subClassOf rico:Activity ,
                              [ rdf:type owl:Restriction ;
                                owl:onProperty :isOrWasProjectPhaseOf ;
                                owl:allValuesFrom :ArchitecturalProject
                              ] ;
              rdfs:comment "Phase of the architectural project, the set of activities within the project usually performed with a particular goal."@en ;
              rdfs:label "Project Phase"@en .


###  https://dmikhaylova.github.io/itdt_ontology/#ProjectRole
:ProjectRole rdf:type owl:Class ;
             rdfs:subClassOf rico:Thing ;
             rdfs:comment "A role in architectural project performed by an architect or an engineer."@en ;
             rdfs:label "Project Role"@en .


###  https://dmikhaylova.github.io/itdt_ontology/#ProjectScale
:ProjectScale rdf:type owl:Class ;
              rdfs:subClassOf rico:Type ;
              rdfs:comment "Categorisation of the project in respect of the area affected by its intervention, where the largest scale project affects a part of territory and the smallest affects only an object."@en ;
              rdfs:isDefinedBy "https://dmikhaylova.github.io/itdt_ontology"@en ;
              rdfs:label "Project Scale"@en ;
              <http://www.w3.org/2004/02/skos/core#example> "design industriale"@it ,
                                                            "general urban planning"@en ,
                                                            "interior design"@en ,
                                                            "progettazione architettonica"@it .


###  https://dmikhaylova.github.io/itdt_ontology/#Report
:Report rdf:type owl:Class ;
        rdfs:subClassOf :WrittenRecord ;
        rdfs:comment "Descriptive document submitted, together with drawings, by an architect to regulating bodies to obtain permission for building or as a part of documents for an architectural competition."@en ;
        rdfs:label "Report"@en .


###  https://dmikhaylova.github.io/itdt_ontology/#Section
:Section rdf:type owl:Class ;
         rdfs:subClassOf :WorkingDrawing ;
         rdfs:comment "Orthographic drawing or work in another media depicting a building, object, or site as if cut through and exposed at one specific plane."@en ;
         rdfs:label "Section"@en .


###  https://dmikhaylova.github.io/itdt_ontology/#SetupStage
:SetupStage rdf:type owl:Class ;
            rdfs:subClassOf :CreativePhase ;
            rdfs:comment "The first stage of the creative phase during which an architect translates the requirements for the building, often written in the form of a list of rooms and their intended functions, into a scheme, configuration of spaces connected to each other. The documents associated with this stage are often ideograms, such as a distribution scheme, that describes synthetically the relations and the necessary functions of contiguity of individual spaces that compose the building."@en ;
            rdfs:label "Setup Stage"@en .


###  https://dmikhaylova.github.io/itdt_ontology/#StructuralPlan
:StructuralPlan rdf:type owl:Class ;
                rdfs:subClassOf :ConstructionDrawing ;
                rdfs:comment "Drawing or work in another medium, often prepared by an engineer, that is  concerned with the load-carrying members of a structure, the plan outline the size and types of materials to be used and the general demands for connections."@en ;
                rdfs:label "Structural Plan"@en .


###  https://dmikhaylova.github.io/itdt_ontology/#VirtualModel
:VirtualModel rdf:type owl:Class ;
              rdfs:subClassOf :Model ;
              rdfs:comment "Architectural models made using software."@en ;
              rdfs:label "Virtual Model"@en .


###  https://dmikhaylova.github.io/itdt_ontology/#WorkingDrawing
:WorkingDrawing rdf:type owl:Class ;
                rdfs:subClassOf :ArchitecturalDrawing ;
                rdfs:comment "A small to medium scale drawing that give a complete graphic representation of the architect’s plans at a scale that is readable but that still shows little detail."@en ;
                rdfs:label "Working Drawing"@en .


###  https://dmikhaylova.github.io/itdt_ontology/#WrittenRecord
:WrittenRecord rdf:type owl:Class ;
               rdfs:subClassOf :ArchitecturalRecord ;
               rdfs:comment "Document that use natural language for communication, with writings on it, created in the process of designing or construction of an architectural project."@en ;
               rdfs:label "Written Record"@en .


###  https://www.ica.org/standards/RiC/ontology#Activity
rico:Activity rdf:type owl:Class ;
              rdfs:subClassOf rico:Event ,
                              [ rdf:type owl:Restriction ;
                                owl:onProperty rico:isOrWasPerformedBy ;
                                owl:allValuesFrom rico:Agent
                              ] ;
              rdfs:comment "The doing of something for some human purpose."@en ;
              rdfs:isDefinedBy <https://www.ica.org/standards/RiC/ontology> ;
              rdfs:label "Activity"@en ;
              <http://www.w3.org/2004/02/skos/core#changeNote> [ ] ;
<http://www.w3.org/2004/02/skos/core#scopeNote> """Activity is a kind of Event. Activity is specifically used to
            designate purposeful human activity. Activity may be understood from two perspectives.
            First it can be understood as leading to an end. The end is the purpose of the Activity,
            or why the Activity is performed. Second, it can be understood in terms of the processes
            that lead to achieving the end, how the end is realized through coordinated actions.
            Purpose and process are complementary understandings of Activity. Together the two
            perspectives address why the Activity is performed, the expected ends or outcomes; and
            how the Activity fulfills the purpose. While activity has an intended end, it also has
            unintended consequences and results, or side-effects. By and large, these may not be the
            focus of the description, but they are, unquestionably, context. |In a corporate or
            government context an Activity may also be called a 'function'. An Activity exists in a
            specific social and cultural context, and within that context is subject to change over
            time. An Activity may be composed of other Activities."""@en ;
rico:RiCCMCorrespondingComponent """Corresponds to RiC-E15 (Activity
            entity)"""@en .


###  https://www.ica.org/standards/RiC/ontology#Agent
rico:Agent rdf:type owl:Class ;
           rdfs:subClassOf rico:Thing ;
           rdfs:comment """A Person, or Group, or an entity created by a Person or Group
            (Mechanism), or a Position, that acts in the world."""@en ;
           rdfs:isDefinedBy <https://www.ica.org/standards/RiC/ontology> ;
           rdfs:label "Agent"@en ;
           <http://www.w3.org/2004/02/skos/core#changeNote> [ ] ,
[ ] ;
<http://www.w3.org/2004/02/skos/core#scopeNote> """An Agent may have one or more identities; an identity is a
            constellation of properties or relations that together “identify” the Agent. A Person or
            Group commonly has one identity, though each also may have one or more alternative
            identities. Such alternative identities may be shared by more than one Person or Group.
            Alternative identities include but are not limited to pseudonyms, heteronyms, DBA (Doing
            Business As), and trade identities. An alternative identity should not be confused with
            a Position in a Group, for example, presidents, prime ministers, governors, popes,
            royalty, or bishops. Nor should an alternative identity be confused with a variant name
            or identifier of the same identity. Agent also includes entities created by a Person or
            Group that act on behalf of the creating Agent in an autonomous or semi-autonomous
            manner. Examples of a Mechanism include software agents, robots, and space and
            underwater probes that generate data (records) in the course of Activity assigned to and
            in conformance with the instructions given to them by the creating Person or
            Group."""@en ;
rico:RiCCMCorrespondingComponent """Corresponds to RiC-E07 (Agent
            entity)"""@en .


###  https://www.ica.org/standards/RiC/ontology#Concept
rico:Concept rdf:type owl:Class ;
             rdfs:subClassOf rico:Thing ;
             rdfs:comment """An idea, unit of thought, abstract cultural object or
            category"""@en ;
             rdfs:isDefinedBy <https://www.ica.org/standards/RiC/ontology> ;
             rdfs:label "Concept"@en .


###  https://www.ica.org/standards/RiC/ontology#CorporateBody
rico:CorporateBody rdf:type owl:Class ;
                   rdfs:subClassOf rico:Group ;
                   rdfs:comment """An organized group of persons that act together as an Agent, and
            that has a recognized legal or social status."""@en ;
                   rdfs:isDefinedBy <https://www.ica.org/standards/RiC/ontology> ;
                   rdfs:label "Corporate Body"@en ;
                   <http://www.w3.org/2004/02/skos/core#changeNote> [ ] ;
<http://www.w3.org/2004/02/skos/core#scopeNote> "Corporate Body is a kind of Group."@en ;
rico:RiCCMCorrespondingComponent """Corresponds to RiC-E11 (Corporate Body
            entity)"""@en .


###  https://www.ica.org/standards/RiC/ontology#Date
rico:Date rdf:type owl:Class ;
          rdfs:subClassOf rico:Thing ;
          rdfs:comment """Chronological information associated with an entity that
            contributes to its identification and contextualization."""@en ;
          rdfs:isDefinedBy <https://www.ica.org/standards/RiC/ontology> ;
          rdfs:label "Date"@en ;
          <http://www.w3.org/2004/02/skos/core#changeNote> [ ] ;
<http://www.w3.org/2004/02/skos/core#scopeNote> """Date includes both single dates, a date range, or a set of
            non-contiguous single dates or date ranges. A date may be represented in natural
            language, based on a digital standard, or both. Digital standard dates will typically be
            based on ISO 8601, or Extended Date-Time Format (EDTF)."""@en ;
rico:RiCCMCorrespondingComponent """Corresponds to RiC-E18 (Date
            entity)"""@en .


###  https://www.ica.org/standards/RiC/ontology#DateRange
rico:DateRange rdf:type owl:Class ;
               rdfs:subClassOf rico:Date ,
                               [ rdf:type owl:Restriction ;
                                 owl:onProperty rico:hasBeginningDate ;
                                 owl:maxQualifiedCardinality "1"^^xsd:nonNegativeInteger ;
                                 owl:onClass rico:SingleDate
                               ] ,
                               [ rdf:type owl:Restriction ;
                                 owl:onProperty rico:hasEndDate ;
                                 owl:maxQualifiedCardinality "1"^^xsd:nonNegativeInteger ;
                                 owl:onClass rico:SingleDate
                               ] ;
               rdfs:comment """Chronological information associated with an entity that
            contributes to its identification and contextualization, that implies or explicitly
            states a start date and end date."""@en ;
               rdfs:isDefinedBy <https://www.ica.org/standards/RiC/ontology> ;
               rdfs:label "Date Range"@en ;
               rico:RiCCMCorrespondingComponent """Corresponds to RiC-E20 (Date Range
            entity)"""@en .


###  https://www.ica.org/standards/RiC/ontology#DateSet
rico:DateSet rdf:type owl:Class ;
             rdfs:subClassOf rico:Date ;
             rdfs:comment "Non-contiguous single dates or date ranges."@en ;
             rdfs:isDefinedBy <https://www.ica.org/standards/RiC/ontology> ;
             rdfs:label "Date Set"@en ;
             <http://www.w3.org/2004/02/skos/core#changeNote> [ ] ;
<http://www.w3.org/2004/02/skos/core#scopeNote> """Primarily used in the description of Record Sets to describe
            dates of member Records"""@en ;
rico:RiCCMCorrespondingComponent """Corresponds to RiC-E21 (Date Set
            entity)"""@en .


###  https://www.ica.org/standards/RiC/ontology#DocumentaryFormType
rico:DocumentaryFormType rdf:type owl:Class ;
                         rdfs:subClassOf rico:Type ,
                                         [ rdf:type owl:Restriction ;
                                           owl:onProperty rico:isDocumentaryFormTypeOf ;
                                           owl:allValuesFrom [ rdf:type owl:Class ;
                                                               owl:unionOf ( rico:Record
                                                                             rico:RecordPart
                                                                           )
                                                             ]
                                         ] ;
                         rdfs:comment """Categorization of the document with respect to its extrinsic and
            intrinsic elements that together communicate its content, administrative and documentary
            context, and authority"""@en ;
                         rdfs:isDefinedBy <https://www.ica.org/standards/RiC/ontology> ;
                         rdfs:label "Documentary Form Type"@en ;
                         <http://www.w3.org/2004/02/skos/core#changeNote> [ ] ;
<http://www.w3.org/2004/02/skos/core#scopeNote> """Documentary Form Type plays an important role in determining
            the type of information a Record may comprise, its status of perfection, and its
            authenticity and reliability. Documentary form types exist in a specific social and
            cultural context, and within that context, are subject to change over
            time"""@en ;
rico:RiCCMCorrespondingComponent """Corresponds to RiC-A17 (Documentary Form Type
            attribute)"""@en .


###  https://www.ica.org/standards/RiC/ontology#Event
rico:Event rdf:type owl:Class ;
           rdfs:subClassOf rico:Thing ;
           rdfs:comment "Something that happens in time and space."@en ;
           rdfs:isDefinedBy <https://www.ica.org/standards/RiC/ontology> ;
           rdfs:label "Event"@en ;
           <http://www.w3.org/2004/02/skos/core#changeNote> [ ] ;
<http://www.w3.org/2004/02/skos/core#scopeNote> """An event may be natural, human, or a combination of natural
            and human. Events have temporal and spatial boundaries. An event may actively involve
            some agent(s) and affect any entity. An event may be discrete, happening at a specific
            moment in time, or may occur over an extended period of time. Events may have events as
            parts, and events may precede or follow one another. Multiple agents may participate in
            the same event, and in different roles. """@en ;
rico:RiCCMCorrespondingComponent """Corresponds to RiC-E14 (Event
            entity)"""@en ;
rico:closeTo """LODE Event class
            (http://linkedevents.org/ontology/#term-Event)"""@en .


###  https://www.ica.org/standards/RiC/ontology#Family
rico:Family rdf:type owl:Class ;
            rdfs:subClassOf rico:Group ;
            rdfs:comment """Two or more persons related by birth, or through marriage,
            adoption, civil union, or other social conventions that bind them together as a socially
            recognized familial group."""@en ;
            rdfs:isDefinedBy <https://www.ica.org/standards/RiC/ontology> ;
            rdfs:label "Family"@en ;
            <http://www.w3.org/2004/02/skos/core#changeNote> [ ] ;
<http://www.w3.org/2004/02/skos/core#scopeNote> """Family is a kind of Group. “Family” is used here as a general
            term that encompasses a wide variety of familial groups. Other types of familial groups
            include Dynasty, Clan, House, Tribe and others. Though family may be a recognized legal
            group in specific contexts, the term may also be used for groups that are socially
            recognized as families. A family may be a group of persons related either by
            consanguinity or affinity or cohabitation or other social conventions. In some context,
            a Family may be legally recognized as Corporate Body. For example, certain North
            American peoples (tribes) retain self-government rights and have jurisdiction over
            defined tribal lands."""@en ;
rico:RiCCMCorrespondingComponent """Corresponds to RiC-E10 (Family
            entity)"""@en .


###  https://www.ica.org/standards/RiC/ontology#Group
rico:Group rdf:type owl:Class ;
           rdfs:subClassOf rico:Agent ;
           owl:disjointWith rico:Person .


###  https://www.ica.org/standards/RiC/ontology#Instantiation
rico:Instantiation rdf:type owl:Class ;
                   rdfs:subClassOf rico:Thing ;
                   rdfs:comment """The inscription of information made by an Agent on a physical
            carrier in any persistent, recoverable form as a means of communicating information
            through time and space."""@en ;
                   rdfs:isDefinedBy <https://www.ica.org/standards/RiC/ontology> ;
                   rdfs:label "Instantiation"@en ;
                   <http://www.w3.org/2004/02/skos/core#changeNote> [ ] ;
<http://www.w3.org/2004/02/skos/core#scopeNote> """A Record or Record Part must have been instantiated at least
            once, though this instantiation may no longer exist at the moment of description. An
            instantiation might also exist at the moment of description, but be destroyed at a later
            moment in time, when, for example, a derived instantiation might become the only
            remaining instantiation. A Record Set may have an instantiation, which is to say that it
            is not a necessary condition. An Instantiation may be derived from another
            Instantiation. A Record Resource may have many Instantiations simultaneously (for
            instance, a record printed and saved in the same time as DOCX and PDF/A would have 3
            concurrent instantiations) or through time (for example, copy of a record). Depending on
            the context, a new instantiation may be seen as a new or as the same record resource.
            During in the process of re-instantiation something is lost and something is preserved,
            but it is up to the context and the Agent that produces or uses that Instantiation to
            assess whether the two instantiations are functionally equivalent or not. For instance,
            a postcard representing a town map from 1874 (Instantiation 1) is digitized and kept as
            a JPEG file (Instantiation 2). The digital copy may be considered as instantiating the
            \"same\" Record by an Agent considering the information transmitted by the Record (e.g.,
            the urban landscape displayed), but as a\" different\" Record by an antiquarian more
            focused on the materiality of the carrier. Successive instantiations may change the
            perceivable boundaries of a Record Resource. For instance, a case file comprising many
            records may be digitized and saved as one single PDF file, which, from management
            perspective, may be treated as one Record. Similarly, a large Record Set (a fonds or a
            series) may be maintained as one database. On the other hand, one record (main document
            and its annexes) may be digitized in separate files and each one may be managed as a
            discrete “physical” item. Instantiations may require mediation to communicate the
            information in the Record Resource. While a traditional Record on paper can simply be
            read by an Agent in order to understand the information, a vinyl recording, a video
            cassette or a digital file needs a device (mediator) to codify or decodify the
            information conveyed. This mediator may imply simple physical components (a turntable
            needle, for example), or a complex gallery of software and hardware elements.
            Instantiations are more than the mere informational content of Record Resource and may
            be the focus of preservation and physical management of records. The use of particular
            document types for records, such as a medieval charter, may have implications for the
            authenticity of the records. Hence, the way a Record Resource is instantiated
            contributes to the contextualizing of the content.record resource is instantiated
            contributes to the contextualizing the content. Distinguishing the message conveyed
            (Record Resource) and its physical representations (Instantiation) allows for the
            efficient management of their descriptions, and preserve information about a Record
            Resource even when no physical representation of it exists or is known to exist anymore.
            The relations between distinct instantiations can then be expressed wherever they
            coexist, and they can be related to the Record Resource they
            instantiate."""@en ;
rico:RiCCMCorrespondingComponent """Corresponds to RiC-E06 (Instantiation
            entity)"""@en ;
rico:closeTo "PREMIS Representation"@en .


###  https://www.ica.org/standards/RiC/ontology#Person
rico:Person rdf:type owl:Class ;
            owl:equivalentClass wd:Q5 ;
            rdfs:subClassOf rico:Agent ;
            rdfs:comment "A human being with a social identity or persona."@en ;
            rdfs:isDefinedBy <https://www.ica.org/standards/RiC/ontology> ;
            rdfs:label "Person"@en ;
            <http://www.w3.org/2004/02/skos/core#changeNote> [ ] ,
[ ] ;
<http://www.w3.org/2004/02/skos/core#scopeNote> """Person is a kind of Agent. Most commonly, a human being
            (biological person) has a single coeval social identity or persona. In everyday
            discourse, this is the “real person.” Less common though not rare, over the course of a
            lifetime, personae in addition to the coeval (or “original”) persona may be associated
            with the human being. Such “alternative personae” are most often created by the original
            person for specific purposes. Under some circumstances, an alternative persona might
            eclipse or replace the original person (Mark Twain eclipsing Samuel Clemens; John Wayne
            eclipsing Marion Mitchell Morrison), that is, the social (shared) alternative identity
            becomes the predominate identity. Less common is whentwo or more persons collaborate to
            create a shared persona. Persona shared by two or more Persons constitute a kind of
            Group. Within the archival context, the original Person generally will be the focus of
            the description, with alternative personae noted. Exceptionally, an alternative persona
            may displace the coeval persona.s."""@en ;
rico:RiCCMCorrespondingComponent """Corresponds to RiC-E08 (Person
            entity)"""@en .


###  https://www.ica.org/standards/RiC/ontology#Place
rico:Place rdf:type owl:Class ;
           rdfs:subClassOf rico:Thing ;
           rdfs:comment "Bounded, named geographic area or region."@en ;
           rdfs:isDefinedBy <https://www.ica.org/standards/RiC/ontology> ;
           rdfs:label "Place"@en ;
           <http://www.w3.org/2004/02/skos/core#changeNote> [ ] ;
<http://www.w3.org/2004/02/skos/core#scopeNote> """A Place may be a jurisdiction, a manmade structure, or a
            natural feature. A manmade structure or natural feature may also be a jurisdiction. A
            Place may be referenced to a Physical Location on the earth, or (if you don't want to
            use the PhysicalLocation class) directly to geographic coordinates. Both jurisdictions
            and natural features are historical entities. A Place thus may have begin and end dates,
            and changing boundaries that result from human or natural events. A Jurisdiction is the
            bounded geographic area within which an Agent has the authority to perform specified
            activities constrained by rules."""@en ;
rico:RiCCMCorrespondingComponent """Corresponds to RiC-E22 (Place
            entity)"""@en .


###  https://www.ica.org/standards/RiC/ontology#Record
rico:Record rdf:type owl:Class ;
            rdfs:subClassOf rico:RecordResource ;
            rdfs:comment """Information inscribed at least once by any method on any
            physical carrier in any persistent, recoverable form by an Agent in the course of life
            or work Activity."""@en ;
            rdfs:isDefinedBy <https://www.ica.org/standards/RiC/ontology> ;
            rdfs:label "Record"@en ;
            <http://www.w3.org/2004/02/skos/core#changeNote> [ ] ,
[ ] ;
<http://www.w3.org/2004/02/skos/core#scopeNote> """Record is a kind of Record Resource. A Record must have or
            have had at least one Instantiation. A Record may have more than one Instantiation. A
            re-instantiation of the record may be considered the same record or a new record,
            depending on the context and of the functions that record serves. Such information may
            serve a variety of purposes, though it always documents or is evidence of
            Activity."""@en ;
rico:RiCCMCorrespondingComponent """Corresponds to RiC-E04 (Record
            entity)"""@en .


###  https://www.ica.org/standards/RiC/ontology#RecordPart
rico:RecordPart rdf:type owl:Class ;
                rdfs:subClassOf rico:Thing .


###  https://www.ica.org/standards/RiC/ontology#RecordResource
rico:RecordResource rdf:type owl:Class ;
                    rdfs:subClassOf rico:Thing ,
                                    [ rdf:type owl:Restriction ;
                                      owl:onProperty rico:hasInstantiation ;
                                      owl:allValuesFrom rico:Instantiation
                                    ] ;
                    rdfs:comment """A Record, Record Set, or Record Part produced or acquired and
            retained by an Agent in the course of Activity."""@en ;
                    rdfs:isDefinedBy <https://www.ica.org/standards/RiC/ontology> ;
                    rdfs:label "Record Resource"@en ;
                    <http://www.w3.org/2004/02/skos/core#changeNote> [ ] ,
[ ] ;
<http://www.w3.org/2004/02/skos/core#scopeNote> """Producing a record resource may imply either its newly
            creation or a reuse of previous existing information by combination, rearrangement,
            selecting, reformatting etc. Records, Record Sets, and Record Parts are all evidence of
            the activities of an Agent. More than one Agent may be involved in the creation of a
            Record Resource. The role of the Agent in creating the Record Resource may take
            different forms, for example, authoring of an individual record, accumulating a set of
            records, or forming a set of records. Though a Record, Record Set, and Record Part,
            under most circumstances, may be easily distinguished from one another, frequently
            identifying the boundary of each and how the “bounded information regions” interrelate,
            may present particular challenges. Documentary Forms provide the rules governing many
            Records, providing criteria for identifying its boundary, and identifying its essential
            Record Parts. Many Records, though, do not have well-established documentary forms,
            particularly electronic records, where it may be difficult to determine whether
            individual elements represented in separate bitstreams are record parts, records, or
            record sets. For example, is a photograph represented independently in a bitstream
            embedded in a text document a Record, or a Record Part ? Or is the same photograph
            attached to an email, maintaining its independent representation, a Record or a Record
            Part? When information is grouped for some purpose, for example, zip or tar “file
            compression” for saving storage space, presents a further challenge. One file comprises
            multiple bitstreams subjected to techniques that remove bits that can be losslessly
            recovered when decompressed. Under what circumstances is such a compressed bitstream a
            Record or a Record Set? Determining when an information object is a Record, Record Part,
            or Record Set is based on perspective and judgement exercised in a particular context.
            In one context, the Agent describing an information object may designate it a Record,
            while another Agent in a different context may designate it a Record Part. Both
            designations are supported by RiC, and the significance of the difference for users of
            the records is ameliorated by the fact that attributes and relations employed in
            describing each of the record entities are shared."""@en ;
rico:RiCCMCorrespondingComponent """Corresponds to RiC-E02 (Record Resource
            entity)"""@en .


###  https://www.ica.org/standards/RiC/ontology#RecordSet
rico:RecordSet rdf:type owl:Class ;
               rdfs:subClassOf rico:RecordResource ;
               rdfs:comment """One or more records that are associated by categorization and/or
            physical aggregation by the creator or other Agent."""@en ;
               rdfs:isDefinedBy <https://www.ica.org/standards/RiC/ontology> ;
               rdfs:label "Record Set"@en ;
               <http://www.w3.org/2004/02/skos/core#changeNote> [ ] ;
<http://www.w3.org/2004/02/skos/core#scopeNote> """Record Set is a kind of Record Resource. The Record members in
            a Record Set may physically reside together, though physical proximity is not essential.
            In a particular context, an Agent (e.g. administrator, records manager, archivist,
            end-user, etc.) may select the Record members of a Record Set based on a shared
            attribute or attributes, or a shared Relation or Relations. The grouping of the Records
            serves a purpose or purposes specific to the context of the Agent. All Record members of
            a Record Set may share the attribute of having been accumulated by the same Agent, or
            all share the same Documentary Form Type and are created over time by the same Activity.
            A Record Set may represent the act of classifying the Records in accordance with a
            formal classification scheme that may be based on Activity, subject, organizational
            structure, or other criteria; an act of archival arrangement (e.g. based on common
            provenance); or some other selection and grouping that fulfils a particular purpose or
            purposes (e.g. a classification that reflects or supports the purposes of a researcher).
            By exception, some Records are brought together based on their not belonging in the
            context of selection to other designated groups: a ‘Miscellaneous’ series, for example.
            A Record Set accumulated by an Agent in the course of life or work Activity should be
            kept in a manner that preserves context and evidential value. Records Sets may also
            contain other Records Sets. Both a Record Set and a Record may simultaneously be a
            member of more than one Record Set, and over the course of its existence, a Record Set
            or Record may be a member of an indeterminate number of Record Sets in an indeterminate
            number of contexts. Record Sets and Records contained within a Record Set may be ordered
            into a sequence based on a common property or relation, or common properties or
            relations (e.g. alphabetical by Agent or related Place name; chronological order by an
            allocated Date); or some other criterion (e.g. an imposed order by
            relevance)."""@en ;
rico:RiCCMCorrespondingComponent """Corresponds to RiC-E03 (Record Set
            entity)"""@en .


###  https://www.ica.org/standards/RiC/ontology#RecordSetType
rico:RecordSetType rdf:type owl:Class ;
                   rdfs:subClassOf rico:Type ,
                                   [ rdf:type owl:Restriction ;
                                     owl:onProperty rico:isRecordSetTypeOf ;
                                     owl:allValuesFrom rico:RecordSet
                                   ] ;
                   rdfs:comment "A broad categorization of the type of Record Set."@en ;
                   rdfs:isDefinedBy <https://www.ica.org/standards/RiC/ontology> ;
                   rdfs:label "Record Set Type"@en ;
                   <http://www.w3.org/2004/02/skos/core#changeNote> [ ] ;
<http://www.w3.org/2004/02/skos/core#scopeNote> """Four instances of Record Set Type are included for now in
            RiC-O; they also are instances of skos:Concept and, as such, part of a SKOS vocabulary.
            Record Set Type may also be used to categorize types of Record Set that have not
            traditionally been considered archival, e.g. search result list."""@en ;
rico:RiCCMCorrespondingComponent """Corresponds to RiC-A36 (Record Set Type
            attribute)"""@en .


###  https://www.ica.org/standards/RiC/ontology#RepresentationType
rico:RepresentationType rdf:type owl:Class ;
                        rdfs:subClassOf rico:Type ,
                                        [ rdf:type owl:Restriction ;
                                          owl:onProperty rico:isRepresentationTypeOf ;
                                          owl:allValuesFrom rico:Instantiation
                                        ] ;
                        rdfs:comment """Categorization of the method of recording the content type of a
            Record Resource."""@en ;
                        rdfs:isDefinedBy <https://www.ica.org/standards/RiC/ontology> ;
                        rdfs:label "Representation Type"@en ;
                        <http://www.w3.org/2004/02/skos/core#changeNote> [ ] ;
<http://www.w3.org/2004/02/skos/core#scopeNote> """Representation Type can be unmediated (which allows humans to
            receive the message communicated without an intermediation of a device) and mediated
            (which needs a device to decode the message). A lot of contemporary mediated types are
            digital. Each Representation Type may present specific features: bit rate for audio,
            resolution for digital images, encoding format for video etc. Depending of the type,
            properties may thus be needed to describe their characteristics. Not be confused with
            Content Type or Carrier Type since the form of representation can be independent of the
            communication or carrier."""@en ;
rico:RiCCMCorrespondingComponent """Corresponds to RiC-A37 (Representation Type
            attribute)"""@en .


###  https://www.ica.org/standards/RiC/ontology#Rule
rico:Rule rdf:type owl:Class .


###  https://www.ica.org/standards/RiC/ontology#SingleDate
rico:SingleDate rdf:type owl:Class ;
                rdfs:subClassOf rico:Date ;
                rdfs:comment """Chronological information associated with an entity that
            contributes to its identification and contextualization, related to a single point in
            time."""@en ;
                rdfs:isDefinedBy <https://www.ica.org/standards/RiC/ontology> ;
                rdfs:label "Single Date"@en ;
                rico:RiCCMCorrespondingComponent """Corresponds to RiC-E19 (SingleDate
            entity)"""@en .


###  https://www.ica.org/standards/RiC/ontology#Thing
rico:Thing rdf:type owl:Class .


###  https://www.ica.org/standards/RiC/ontology#Type
rico:Type rdf:type owl:Class ;
          rdfs:subClassOf rico:Concept ;
          rdfs:comment """A superclass for any category of some thing. A type
            characterizes an entity."""@en ;
          rdfs:isDefinedBy <https://www.ica.org/standards/RiC/ontology> ;
          rdfs:label "Type"@en .


###  https://www.wikidata.org/wiki/Q12737077
wd:Q12737077 rdf:type owl:Class ;
             rdfs:label "occupation"@en .


###  https://www.wikidata.org/wiki/Q5
wd:Q5 rdf:type owl:Class ;
      rdfs:label "human"@en .


#################################################################
#    Individuals
#################################################################

###  http://culturaitalia.it/pico/thesaurus/4.1#abitazioni
<http://culturaitalia.it/pico/thesaurus/4.1#abitazioni> rdf:type owl:NamedIndividual ;
                                                        owl:sameAs :residentialUse ;
                                                        rdfs:label "abitazioni"@it ,
                                                                   "dwellings"@en .


###  http://culturaitalia.it/pico/thesaurus/4.1#edifici_industriali
<http://culturaitalia.it/pico/thesaurus/4.1#edifici_industriali> rdf:type owl:NamedIndividual ;
                                                                 owl:sameAs :industrialUse ;
                                                                 rdfs:label "industrial buildings"@en .


###  https://dmikhaylova.github.io/itdt_ontology#artisanalLaboratory
:artisanalLaboratory rdf:type owl:NamedIndividual ,
                              :FunctionalBuildingType ;
                     rdfs:label "artisanal laboratories"@en ;
                     <http://www.w3.org/2004/02/skos/core#broader> :industrialUse .


###  https://dmikhaylova.github.io/itdt_ontology#bank
:bank rdf:type owl:NamedIndividual ,
               :FunctionalBuildingType ;
      rdfs:label "banks"@en ;
      <http://www.w3.org/2004/02/skos/core#broader> :executiveUse .


###  https://dmikhaylova.github.io/itdt_ontology#fair
:fair rdf:type owl:NamedIndividual ,
               :FunctionalBuildingType ;
      rdfs:label "fair or exibition"@en ;
      <http://www.w3.org/2004/02/skos/core#broader> :commercialUse .


###  https://dmikhaylova.github.io/itdt_ontology#hotel
:hotel rdf:type owl:NamedIndividual ,
                :FunctionalBuildingType ;
       rdfs:label "hotels"@en ;
       <http://www.w3.org/2004/02/skos/core#broader> :touristicUse .


###  https://dmikhaylova.github.io/itdt_ontology#industry
:industry rdf:type owl:NamedIndividual ,
                   :FunctionalBuildingType ;
          rdfs:comment "industrial structures"@en ;
          <http://www.w3.org/2004/02/skos/core#broader> :industrialUse .


###  https://dmikhaylova.github.io/itdt_ontology#insurance
:insurance rdf:type owl:NamedIndividual ,
                    :FunctionalBuildingType ;
           rdfs:label "insuarance buildings"@en ;
           <http://www.w3.org/2004/02/skos/core#broader> :executiveUse .


###  https://dmikhaylova.github.io/itdt_ontology#market
:market rdf:type owl:NamedIndividual ,
                 :FunctionalBuildingType ;
        rdfs:label "markets"@en ;
        <http://www.w3.org/2004/02/skos/core#broader> :commercialUse .


###  https://dmikhaylova.github.io/itdt_ontology#officePrivate
:officePrivate rdf:type owl:NamedIndividual ,
                        :FunctionalBuildingType ;
               rdfs:label "private offices"@en ;
               <http://www.w3.org/2004/02/skos/core#broader> :executiveUse .


###  https://dmikhaylova.github.io/itdt_ontology#officeService
:officeService rdf:type owl:NamedIndividual ,
                        :FunctionalBuildingType ;
               rdfs:label "offices of service companies"@en ;
               <http://www.w3.org/2004/02/skos/core#broader> :executiveUse .


###  https://dmikhaylova.github.io/itdt_ontology#researchCenter
:researchCenter rdf:type owl:NamedIndividual ,
                         :FunctionalBuildingType ;
                rdfs:label "research centres"@en ;
                <http://www.w3.org/2004/02/skos/core#broader> :executiveUse .


###  https://dmikhaylova.github.io/itdt_ontology#residence
:residence rdf:type owl:NamedIndividual ,
                    :FunctionalBuildingType ;
           rdfs:label "touristic residences"@en ;
           <http://www.w3.org/2004/02/skos/core#broader> :touristicUse .


###  https://dmikhaylova.github.io/itdt_ontology#restaurant
:restaurant rdf:type owl:NamedIndividual ,
                     :FunctionalBuildingType ;
            rdfs:label "restaurants"@en ;
            <http://www.w3.org/2004/02/skos/core#broader> :commercialUse .


###  https://dmikhaylova.github.io/itdt_ontology#shop
:shop rdf:type owl:NamedIndividual ,
               :FunctionalBuildingType ;
      rdfs:label "shops"@en ;
      <http://www.w3.org/2004/02/skos/core#broader> :commercialUse .


###  https://dmikhaylova.github.io/itdt_ontology#warehouse
:warehouse rdf:type owl:NamedIndividual ,
                    :FunctionalBuildingType ;
           rdfs:label "warehouses"@en ;
           <http://www.w3.org/2004/02/skos/core#broader> :industrialUse .


###  https://dmikhaylova.github.io/itdt_ontology#workshop
:workshop rdf:type owl:NamedIndividual ,
                   :FunctionalBuildingType ;
          rdfs:label "workshops"@en ;
          <http://www.w3.org/2004/02/skos/core#broader> :industrialUse .


###  https://dmikhaylova.github.io/itdt_ontology/#ProjectScales
:ProjectScales rdf:type owl:NamedIndividual ,
                        <http://www.w3.org/2004/02/skos/core#ConceptScheme> ;
               rdfs:label "Project Scales"@en .


###  https://dmikhaylova.github.io/itdt_ontology/#agriculturalUse
:agriculturalUse rdf:type owl:NamedIndividual ,
                          <http://www.w3.org/2004/02/skos/core#Concept> ,
                          :FunctionalBuildingType ;
                 rdfs:label "agricultural use"@en ;
                 owl:sameAs "http://vocab.getty.edu/aat/300004895" ;
                 <http://www.w3.org/2004/02/skos/core#inScheme> :functionalBuildingTypes .


###  https://dmikhaylova.github.io/itdt_ontology/#architecturalDesign
:architecturalDesign rdf:type owl:NamedIndividual ,
                              <http://www.w3.org/2004/02/skos/core#Concept> ,
                              :ProjectScale ;
                     rdfs:label "architectural design"@en ;
                     <http://www.w3.org/2004/02/skos/core#inScheme> :ProjectScales .


###  https://dmikhaylova.github.io/itdt_ontology/#blockAppartmentBuilding
:blockAppartmentBuilding rdf:type owl:NamedIndividual ,
                                  <http://www.w3.org/2004/02/skos/core#Concept> ,
                                  :FormalBuildingType ;
                         rdfs:label "block appartment building"@en ;
                         <http://www.w3.org/2004/02/skos/core#inScheme> :formalBuildingTypes .


###  https://dmikhaylova.github.io/itdt_ontology/#commercialUse
:commercialUse rdf:type owl:NamedIndividual ,
                        <http://www.w3.org/2004/02/skos/core#Concept> ,
                        :FunctionalBuildingType ;
               rdfs:label "commercial use"@en ;
               owl:sameAs "http://vocab.getty.edu/aat/300005147" ;
               <http://www.w3.org/2004/02/skos/core#inScheme> :functionalBuildingTypes .


###  https://dmikhaylova.github.io/itdt_ontology/#courtyardHouse
:courtyardHouse rdf:type owl:NamedIndividual ,
                         <http://www.w3.org/2004/02/skos/core#Concept> ,
                         :FormalBuildingType ;
                rdfs:label "courtyard house"@en ;
                <http://www.w3.org/2004/02/skos/core#inScheme> :formalBuildingTypes .


###  https://dmikhaylova.github.io/itdt_ontology/#executiveUse
:executiveUse rdf:type owl:NamedIndividual ,
                       <http://www.w3.org/2004/02/skos/core#Concept> ,
                       :FunctionalBuildingType ;
              rdfs:label "executive use"@en ;
              <http://www.w3.org/2004/02/skos/core#inScheme> :functionalBuildingTypes .


###  https://dmikhaylova.github.io/itdt_ontology/#formalBuildingTypes
:formalBuildingTypes rdf:type owl:NamedIndividual ,
                              <http://www.w3.org/2004/02/skos/core#ConceptScheme> ;
                     rdfs:label "Formal Building Types"@en ,
                                "Tipologia edilizia"@it .


###  https://dmikhaylova.github.io/itdt_ontology/#functionalBuildingTypes
:functionalBuildingTypes rdf:type owl:NamedIndividual ,
                                  <http://www.w3.org/2004/02/skos/core#ConceptScheme> ;
                         rdfs:label "Destinazioni d'uso"@it ,
                                    "Functional Building Types"@en .


###  https://dmikhaylova.github.io/itdt_ontology/#generalPlanning
:generalPlanning rdf:type owl:NamedIndividual ,
                          <http://www.w3.org/2004/02/skos/core#Concept> ,
                          :ProjectScale ;
                 rdfs:label "general planning"@en ;
                 <http://www.w3.org/2004/02/skos/core#inScheme> :ProjectScales .


###  https://dmikhaylova.github.io/itdt_ontology/#guardRailHouses
:guardRailHouses rdf:type owl:NamedIndividual ,
                          <http://www.w3.org/2004/02/skos/core#Concept> ,
                          :FormalBuildingType ;
                 rdfs:label "guard rail house"@en ;
                 <http://www.w3.org/2004/02/skos/core#inScheme> :formalBuildingTypes .


###  https://dmikhaylova.github.io/itdt_ontology/#implementationPlanning
:implementationPlanning rdf:type owl:NamedIndividual ,
                                 <http://www.w3.org/2004/02/skos/core#Concept> ,
                                 :ProjectScale ;
                        rdfs:label "implementation planning"@en ;
                        <http://www.w3.org/2004/02/skos/core#inScheme> :ProjectScales .


###  https://dmikhaylova.github.io/itdt_ontology/#industrialUse
:industrialUse rdf:type owl:NamedIndividual ,
                        <http://www.w3.org/2004/02/skos/core#Concept> ,
                        :FunctionalBuildingType ;
               rdfs:label "industrial and artisanal use"@en ;
               owl:sameAs "http://vocab.getty.edu/aat/300121918" ;
               <http://www.w3.org/2004/02/skos/core#inScheme> :functionalBuildingTypes .


###  https://dmikhaylova.github.io/itdt_ontology/#interiorDesign
:interiorDesign rdf:type owl:NamedIndividual ,
                         <http://www.w3.org/2004/02/skos/core#Concept> ,
                         :ProjectScale ;
                rdfs:label "interior and industrial design"@en ;
                <http://www.w3.org/2004/02/skos/core#inScheme> :ProjectScales .


###  https://dmikhaylova.github.io/itdt_ontology/#isolatedHouse
:isolatedHouse rdf:type owl:NamedIndividual ,
                        <http://www.w3.org/2004/02/skos/core#Concept> ,
                        :FormalBuildingType ;
               rdfs:label "isolated house"@en ;
               <http://www.w3.org/2004/02/skos/core#inScheme> :formalBuildingTypes .


###  https://dmikhaylova.github.io/itdt_ontology/#multiFamilyHouse
:multiFamilyHouse rdf:type owl:NamedIndividual ,
                           <http://www.w3.org/2004/02/skos/core#Concept> ,
                           :FormalBuildingType ;
                  rdfs:label "multifamily house"@en .


###  https://dmikhaylova.github.io/itdt_ontology/#projectRoles
:projectRoles rdf:type owl:NamedIndividual ,
                       <http://www.w3.org/2004/02/skos/core#ConceptScheme> ;
              rdfs:label "Project Roles"@en .


###  https://dmikhaylova.github.io/itdt_ontology/#publicUse
:publicUse rdf:type owl:NamedIndividual ,
                    <http://www.w3.org/2004/02/skos/core#Concept> ,
                    :FunctionalBuildingType ;
           rdfs:label "public use"@en ;
           owl:sameAs "http://vocab.getty.edu/aat/300008059" ;
           <http://www.w3.org/2004/02/skos/core#inScheme> :functionalBuildingTypes .


###  https://dmikhaylova.github.io/itdt_ontology/#residentialUse
:residentialUse rdf:type owl:NamedIndividual ,
                         <http://www.w3.org/2004/02/skos/core#Concept> ,
                         :FunctionalBuildingType ;
                rdfs:label "residential use"@en ;
                owl:sameAs "http://vocab.getty.edu/aat/300257729" ;
                <http://www.w3.org/2004/02/skos/core#inScheme> :functionalBuildingTypes .


###  https://dmikhaylova.github.io/itdt_ontology/#restorationOrRenovation
:restorationOrRenovation rdf:type owl:NamedIndividual ,
                                  <http://www.w3.org/2004/02/skos/core#Concept> ,
                                  :ProjectScale ;
                         rdfs:label "restoration or renovation"@en ;
                         <http://www.w3.org/2004/02/skos/core#inScheme> :ProjectScales .


###  https://dmikhaylova.github.io/itdt_ontology/#rowAppartmentBuilding
:rowAppartmentBuilding rdf:type owl:NamedIndividual ,
                                <http://www.w3.org/2004/02/skos/core#Concept> ,
                                :FormalBuildingType ;
                       rdfs:label "row appartment building"@en ;
                       owl:sameAs "http://vocab.getty.edu/aat/300005672" ;
                       <http://www.w3.org/2004/02/skos/core#inScheme> :formalBuildingTypes .


###  https://dmikhaylova.github.io/itdt_ontology/#terracedHouse
:terracedHouse rdf:type owl:NamedIndividual ,
                        <http://www.w3.org/2004/02/skos/core#Concept> ,
                        :FormalBuildingType ;
               rdfs:label "terraced house"@en ;
               owl:sameAs "http://vocab.getty.edu/page/aat/300132989" ;
               <http://www.w3.org/2004/02/skos/core#definition> "Formal type of residential building that applies to houses that are composed by  a series of housing units joined side by side, but not having any other dwellings nor above nor below."@en ;
               <http://www.w3.org/2004/02/skos/core#inScheme> :formalBuildingTypes .


###  https://dmikhaylova.github.io/itdt_ontology/#touristicUse
:touristicUse rdf:type owl:NamedIndividual ,
                       <http://www.w3.org/2004/02/skos/core#Concept> ,
                       :FunctionalBuildingType ;
              rdfs:label "touristic use"@en ;
              owl:sameAs "http://vocab.getty.edu/aat/300164125" ;
              <http://www.w3.org/2004/02/skos/core#inScheme> :functionalBuildingTypes .


###  https://dmikhaylova.github.io/itdt_ontology/#towerAppartmentBuilding
:towerAppartmentBuilding rdf:type owl:NamedIndividual ,
                                  <http://www.w3.org/2004/02/skos/core#Concept> ,
                                  :FormalBuildingType ;
                         rdfs:label "tower appartment building"@en ;
                         owl:sameAs "http://vocab.getty.edu/aat/300004811" ;
                         <http://www.w3.org/2004/02/skos/core#inScheme> :formalBuildingTypes .


###  https://www.ica.org/standards/RiC/vocabularies/documentaryFormTypes
<https://www.ica.org/standards/RiC/vocabularies/documentaryFormTypes> rdf:type owl:NamedIndividual ,
                                                                               <http://www.w3.org/2004/02/skos/core#ConceptScheme> ;
                                                                      dc:creator """International Coucil on Archives Expert Group on Archival
            Description (ICA EGAD)"""@en ;
                                                                      dc:title """International Council on Archives Records in Contexts Vocabulary for
            Documentary Form Types"""@en ;
                                                                      rdfs:label "Documentary Form Types"@en ;
                                                                      <http://www.w3.org/2004/02/skos/core#definition> """A vocabulary that includes documentary form
            types"""@en .


###  https://www.ica.org/standards/RiC/vocabularies/recordSetTypes
<https://www.ica.org/standards/RiC/vocabularies/recordSetTypes> rdf:type owl:NamedIndividual ,
                                                                         <http://www.w3.org/2004/02/skos/core#ConceptScheme> ;
                                                                dc:creator """International Coucil on Archives Expert Group on Archival
            Description (ICA EGAD)"""@en ;
                                                                dc:title """International Council on Archives Records in Contexts Vocabulary for
            Record Set Types"""@en ;
                                                                rdfs:label "Record Set Types"@en ;
                                                                <http://www.w3.org/2004/02/skos/core#definition> "A vocabulary on Record Set types"@en .


###  https://www.ica.org/standards/RiC/vocabularies/recordSetTypes#File
<https://www.ica.org/standards/RiC/vocabularies/recordSetTypes#File> rdf:type owl:NamedIndividual ,
                                                                              <http://www.w3.org/2004/02/skos/core#Concept> ;
                                                                     rdfs:label "file"@en ;
                                                                     <http://www.w3.org/2004/02/skos/core#definition> """An organized unit of documents grouped together either for
            current use by the creator or in the process of archival arrangement, because they
            relate to the same subject, activity, or transaction. A file is usually the basic unit
            within a record series. (From ICA ISAD(G))"""@en ;
                                                                     <http://www.w3.org/2004/02/skos/core#inScheme> <https://www.ica.org/standards/RiC/vocabularies/recordSetTypes> ;
                                                                     <http://www.w3.org/2004/02/skos/core#prefLabel> "file"@en .


###  https://www.ica.org/standards/RiC/vocabularies/recordSetTypes#Fonds
<https://www.ica.org/standards/RiC/vocabularies/recordSetTypes#Fonds> rdf:type owl:NamedIndividual ,
                                                                               <http://www.w3.org/2004/02/skos/core#Concept> ;
                                                                      rdfs:label "fonds"@en ;
                                                                      <http://www.w3.org/2004/02/skos/core#definition> """The whole of the records, regardless of form or medium,
            organically created and/or accumulated and used by a particular person, family, or
            corporate body in the course of that creator's activities and functions. (From ICA
            ISAD(G))"""@en ;
                                                                      <http://www.w3.org/2004/02/skos/core#inScheme> <https://www.ica.org/standards/RiC/vocabularies/recordSetTypes> ;
                                                                      <http://www.w3.org/2004/02/skos/core#prefLabel> "fonds"@en .


###  https://www.ica.org/standards/RiC/vocabularies/recordSetTypes#Series
<https://www.ica.org/standards/RiC/vocabularies/recordSetTypes#Series> rdf:type owl:NamedIndividual ,
                                                                                <http://www.w3.org/2004/02/skos/core#Concept> ;
                                                                       rdfs:label "series"@en ;
                                                                       <http://www.w3.org/2004/02/skos/core#definition> """Documents arranged in accordance with a filing system or
            maintained as a unit because they result from the same accumulation or filing process,
            or the same activity; have a particular form; or because of some other relationship
            arising out of their creation, receipt, or use. A series is also known as a records
            series. (From ICA ISAD(G))"""@en ;
                                                                       <http://www.w3.org/2004/02/skos/core#inScheme> <https://www.ica.org/standards/RiC/vocabularies/recordSetTypes> ;
                                                                       <http://www.w3.org/2004/02/skos/core#prefLabel> "series"@en .


#################################################################
#    General axioms
#################################################################

[ rdf:type owl:AllDisjointClasses ;
  owl:members ( :AcceptancePhase
                :AnalysisPhase
                :CreativePhase
                :ExecutionPhase
                :FollowUpPhase
              )
] .


[ rdf:type owl:AllDisjointClasses ;
  owl:members ( :BidPhase
                :ConstructionPhase
                :PermitStage
              )
] .


[ rdf:type owl:AllDisjointClasses ;
  owl:members ( :ConciseIdeaStage
                :DevelopmentStage
                :SetupStage
              )
] .


[ rdf:type owl:AllDisjointClasses ;
  owl:members ( :GraphicalRecord
                :Model
                :WrittenRecord
              )
] .


[ rdf:type owl:AllDifferent ;
  owl:distinctMembers ( :agriculturalUse
                        :commercialUse
                        :executiveUse
                        :industrialUse
                        :publicUse
                        :residentialUse
                        :touristicUse
                      )
] .


[ rdf:type owl:AllDifferent ;
  owl:distinctMembers ( :blockAppartmentBuilding
                        :courtyardHouse
                        :guardRailHouses
                        :isolatedHouse
                        :rowAppartmentBuilding
                        :terracedHouse
                        :towerAppartmentBuilding
                      )
] .


[ rdf:type owl:AllDifferent ;
  owl:distinctMembers ( :blockAppartmentBuilding
                        :courtyardHouse
                        :multiFamilyHouse
                        :rowAppartmentBuilding
                        :terracedHouse
                        :towerAppartmentBuilding
                      )
] .


[ rdf:type owl:AllDifferent ;
  owl:distinctMembers ( :industrialUse
                        :residentialUse
                      )
] .


[ rdf:type owl:AllDifferent ;
  owl:distinctMembers ( :isolatedHouse
                        :multiFamilyHouse
                      )
] .


###  Generated by the OWL API (version 4.5.9.2019-02-01T07:24:44Z) https://github.com/owlcs/owlapi
